ported general_atomics
Nonexpansiveness support still needs work.

atomics/general_atomics.v
@@ -1,7 +1,5 @@
-From VST.veric Require Import rmaps compcert_rmaps.
-Require Export iris.bi.lib.atomic.
-Require Export VST.veric.bi.
-From VST.concurrency Require Export ghosts conclib invariants fupd.
+Require Export iris.algebra.list iris.bi.lib.atomic.
+From VST.concurrency Require Export conclib.
 Require Import VST.floyd.library.
 Require Export VST.zlist.sublist.
 Require Import Program.Equality.
@@ -16,24 +14,26 @@ Definition tele_unwrap {A} (x : tele_arg (TeleS (fun _ : A => TeleO))) :=
   | TeleArgCons x _ => x
   end.
 
-Definition atomic_shift {A B} (a : A -> mpred) Eo Ei (b : A -> B -> mpred) (Q : B -> mpred) : mpred :=
-  @atomic_update mpredI _ [tele _ : A] [tele _ : B] Eo Ei (λ.. x, a (tele_unwrap x)) (λ.. x y, b (tele_unwrap x) (tele_unwrap y)) (λ.. x y, Q (tele_unwrap y)).
+Context `{!VSTGS OK_ty Σ}.
+
+Definition atomic_shift {A B} (a : A -d> mpred) Eo Ei (b : A -d> B -d> mpred) (Q : B -d> mpred) : mpred :=
+  atomic_update(TA := [tele _ : A]) (TB := [tele _ : B]) Eo Ei (λ.. x, a (tele_unwrap x)) (λ.. x y, b (tele_unwrap x) (tele_unwrap y)) (λ.. x y, Q (tele_unwrap y)).
 
 Lemma atomic_commit_fupd : forall {A B} (a : A -> mpred) Eo Ei (b : A -> B -> mpred) (Q : B -> mpred) R R',
-  (forall x, R * a x |-- |==> (EX y, b x y * R' y)) ->
-  atomic_shift a Eo Ei b Q * R |-- |={Eo}=> (EX y, Q y * R' y).
+  (forall x, R ∗ a x ⊢ |==> (∃ y, b x y ∗ R' y)) ->
+  atomic_shift a Eo Ei b Q ∗ R ⊢ |={Eo}=> (∃ y, Q y ∗ R' y).
 Proof.
   intros.
   iIntros "[AS R]".
-  unfold atomic_shift. 
+  unfold atomic_shift.
   iMod "AS" as (x) "[a [_ commit]]"; simpl.
   iMod (H with "[$R $a]") as (y) "[b Q]".
   iExists y; iMod ("commit" with "b") as "$"; auto.
 Qed.
 
 Lemma atomic_rollback_fupd : forall {A B} (a : A -> mpred) Eo Ei (b : A -> B -> mpred) (Q : B -> mpred) R R',
-  (forall x, R * a x |-- |==> a x * R') ->
-  atomic_shift a Eo Ei b Q * R |-- |={Eo}=> atomic_shift a Eo Ei b Q * R'.
+  (forall x, R ∗ a x ⊢ |==> a x ∗ R') ->
+  atomic_shift a Eo Ei b Q ∗ R ⊢ |={Eo}=> atomic_shift a Eo Ei b Q ∗ R'.
 Proof.
   intros.
   iIntros "[AS R]".
@@ -45,18 +45,18 @@ Qed.
 
 Lemma atomic_shift_mask_weaken {A B} Eo1 Eo2 Ei a (b : A -> B -> mpred) Q :
   Eo1 ⊆ Eo2 ->
-  atomic_shift a Eo1 Ei b Q |-- atomic_shift a Eo2 Ei b Q.
+  atomic_shift a Eo1 Ei b Q ⊢ atomic_shift a Eo2 Ei b Q.
 Proof.
   intros; unfold atomic_shift.
-  apply atomic_update_mask_weaken; auto.
+  iApply atomic_update_mask_weaken; auto.
 Qed.
 
 (* use iInv instead of applying this lemma *)
 Lemma inv_atomic_shift : forall {A B} a Eo Ei (b : A -> B -> mpred) Q N R P
   (Hi : ↑N ⊆ Eo) (Hio : Ei ⊆ Eo ∖ ↑N)
-  (Ha1 : (inv N R * |>R |-- |={Eo ∖ ↑N}=> EX x, a x * ((a x -* |={Ei}=> |>R) &&
-    (ALL y, |> P * b x y -* |={Ei}=> |>R * Q y)))),
-  inv N R * |> P |-- atomic_shift a Eo Ei b Q.
+  (Ha1 : (inv N R ∗ ▷R ⊢ |={Eo ∖ ↑N}=> ∃ x, a x ∗ ((a x -∗ |={Ei}=> ▷R) ∧
+    (∀ y, ▷ P ∗ b x y -∗ |={Ei}=> ▷R ∗ Q y)))),
+  inv N R ∗ ▷ P ⊢ atomic_shift a Eo Ei b Q.
 Proof.
   intros; unfold atomic_shift.
   iIntros "[#I P]". iAuIntro.
@@ -64,7 +64,7 @@ Proof.
   iInv "I" as "R" "Hclose".
   iMod (Ha1 with "[$I $R]") as (x) "(a & shift)".
   iExists x; iFrame.
-  iApply fupd_mask_intro; first done.
+  iApply fupd_mask_intro.
   iIntros "Hclose'"; iSplit.
   - iIntros "a"; iMod ("shift" with "a") as "R".
     iMod "Hclose'"; iMod ("Hclose" with "R"); auto.
@@ -73,27 +73,19 @@ Proof.
     iMod "Hclose'"; iMod ("Hclose" with "R"); auto.
 Qed.
 
-Lemma atomic_shift_nonexpansive : forall {A B} n a Eo Ei (b : A -> B -> mpred) Q,
-  approx n (atomic_shift a Eo Ei b Q) =
-  approx n (atomic_shift (fun x => approx n (a x)) Eo Ei (fun x y => approx n (b x y)) (fun y => approx n (Q y))).
+#[global] Instance atomic_shift_nonexpansive : forall {A B} n,
+  Proper (dist n ==> eq ==> eq ==> dist n ==> dist n ==> dist n) (@atomic_shift A B).
 Proof.
-  intros; unfold atomic_shift.
-  destruct n as [|n].
-  { rewrite !approx_0; auto. }
-  unshelve eapply (atomic_update_ne(TA := TeleS (fun _ => TeleO)) _ _ n (λ.. x : [tele _ : A], a (tele_unwrap x))).
-  { intros [? []]; hnf; simpl.
-    rewrite approx_idem; auto. }
-  { intros [? []] [? []]; hnf; simpl.
-    rewrite approx_idem; auto. }
-  { intros [? []] [? []]; hnf; simpl.
-    rewrite approx_idem; auto. }
+  repeat intro.
+  rewrite /atomic_shift /=.
+  subst; apply atomic_update_ne; intros []; solve_proper.
 Qed.
 
 Lemma atomic_shift_derives_frame : forall {A A' B B'} (a : A -> mpred) (a' : A' -> mpred) Eo Ei
   (b : A -> B -> mpred) (b' : A' -> B' -> mpred) (Q : B -> mpred) (Q' : B' -> mpred) R
-  (Ha : (forall x, a x * |>R |-- |={Ei}=> EX x' : A', a' x' *
-    ((a' x' -* |={Ei}=> a x * |>R) && ALL y' : _, b' x' y' -* (|={Ei}=> EX y : _, b x y * (Q y -* |={Eo}=> Q' y'))))),
-  atomic_shift a Eo Ei b Q * |>R |-- atomic_shift a' Eo Ei b' Q'.
+  (Ha : (forall x, a x ∗ ▷R ⊢ |={Ei}=> ∃ x' : A', a' x' ∗
+    ((a' x' -∗ |={Ei}=> a x ∗ ▷R) ∧ ∀ y' : _, b' x' y' -∗ (|={Ei}=> ∃ y : _, b x y ∗ (Q y -∗ |={Eo}=> Q' y'))))),
+  atomic_shift a Eo Ei b Q ∗ ▷R ⊢ atomic_shift a' Eo Ei b' Q'.
 Proof.
   intros; unfold atomic_shift.
   iIntros "[AU P]". iAuIntro.
@@ -112,9 +104,9 @@ Qed.
 
 Lemma atomic_shift_derives : forall {A A' B B'} (a : A -> mpred) (a' : A' -> mpred) Eo Ei
   (b : A -> B -> mpred) (b' : A' -> B' -> mpred) (Q : B -> mpred) (Q' : B' -> mpred)
-  (Ha : (forall x, a x  |-- |={Ei}=> EX x' : A', a' x' *
-    ((a' x' -* |={Ei}=> a x) && ALL y' : _, b' x' y' -* (|={Ei}=> EX y : _, b x y * (Q y -* |={Eo}=> Q' y'))))),
-  atomic_shift a Eo Ei b Q |-- atomic_shift a' Eo Ei b' Q'.
+  (Ha : (forall x, a x  ⊢ |={Ei}=> ∃ x' : A', a' x' ∗
+    ((a' x' -∗ |={Ei}=> a x) ∧ ∀ y' : _, b' x' y' -∗ (|={Ei}=> ∃ y : _, b x y ∗ (Q y -∗ |={Eo}=> Q' y'))))),
+  atomic_shift a Eo Ei b Q ⊢ atomic_shift a' Eo Ei b' Q'.
 Proof.
   intros; unfold atomic_shift.
   iIntros "AU". iAuIntro.
@@ -129,9 +121,9 @@ Qed.
 
 Lemma atomic_shift_derives' : forall {A A' B} (a : A -> mpred) (a' : A' -> mpred) Eo Ei
   (b : A -> B -> mpred) (b' : A' -> B -> mpred) (Q : B -> mpred)
-  (Ha : (forall x, a x |-- |={Ei}=> EX x' : A', a' x' *
-    ((a' x' -* |={Ei}=> a x) && ALL y : _, b' x' y -* |={Ei}=> b x y))),
-  atomic_shift a Eo Ei b Q |-- atomic_shift a' Eo Ei b' Q.
+  (Ha : (forall x, a x ⊢ |={Ei}=> ∃ x' : A', a' x' ∗
+    ((a' x' -∗ |={Ei}=> a x) ∧ ∀ y : _, b' x' y -∗ |={Ei}=> b x y))),
+  atomic_shift a Eo Ei b Q ⊢ atomic_shift a' Eo Ei b' Q.
 Proof.
   intros; apply atomic_shift_derives.
   iIntros (x) "a"; iMod (Ha with "a") as (x') "[a H]".
@@ -145,10 +137,10 @@ Proof.
 Qed.
 
 Lemma atomic_shift_derives_simple : forall {A B} (a a' : A -> mpred) Eo Ei (b b' : A -> B -> mpred) (Q : B -> mpred)
-  (Ha1 : forall x, a x |-- |={Ei}=> a' x)
-  (Ha2 : forall x, a' x |-- |={Ei}=> a x)
-  (Hb : forall x y, b' x y |-- |={Ei}=> b x y),
-  atomic_shift a Eo Ei b Q |-- atomic_shift a' Eo Ei b' Q.
+  (Ha1 : forall x, a x ⊢ |={Ei}=> a' x)
+  (Ha2 : forall x, a' x ⊢ |={Ei}=> a x)
+  (Hb : forall x y, b' x y ⊢ |={Ei}=> b x y),
+  atomic_shift a Eo Ei b Q ⊢ atomic_shift a' Eo Ei b' Q.
 Proof.
   intros; apply atomic_shift_derives'; intros.
   iIntros "a"; iExists x; iMod (Ha1 with "a") as "$".
@@ -158,7 +150,7 @@ Proof.
 Qed.
 
 Lemma atomic_shift_exists : forall {A B} a Eo Ei (b : A -> B -> mpred) Q,
-  atomic_shift (fun (_ : unit) => EX x : A, a x) Eo Ei (fun (_ : unit) => EX x : A, b x) Q |-- atomic_shift a Eo Ei b Q.
+  atomic_shift (fun (_ : unit) => ∃ x : A, a x) Eo Ei (fun (_ : unit) y => ∃ x : A, b x y) Q ⊢ atomic_shift a Eo Ei b Q.
 Proof.
   intros; unfold atomic_shift.
   iIntros "AU". iAuIntro.
@@ -169,11 +161,9 @@ Proof.
   iIntros "!>"; iSplit.
   - iIntros "a !>".
     iSplitR ""; auto.
-    iExists x; auto.
   - iIntros (y) "b !>".
     iRight; iExists y.
     iSplitR ""; auto.
-    iExists x; auto.
 Qed.
 
 End atomicity.
@@ -181,1148 +171,528 @@ End atomicity.
 Global Hint Resolve empty_subseteq : core.
 
 Definition atomic_spec_type W T := ProdType W (ArrowType (ConstType T) Mpred).
-
-Definition super_non_expansive_a {A W} (a : forall ts : list Type, functors.MixVariantFunctor._functor
-  (dependent_type_functor_rec ts W) (predicates_hered.pred rmap) -> A ts -> predicates_hered.pred rmap) :=
-  forall n ts w x, approx n (a ts w x) =
-  approx n (a ts (functors.MixVariantFunctor.fmap (dependent_type_functor_rec ts W) (approx n) (approx n) w) x).
-
-Definition super_non_expansive_E {W} (E : forall ts : list Type, dependent_type_functor_rec ts W (predicates_hered.pred rmap) -> coPset) :=
-  forall n ts w, E ts w = E ts (functors.MixVariantFunctor.fmap (dependent_type_functor_rec ts W) (approx n) (approx n) w).
-
-Definition super_non_expansive_b {A B W} (b : forall ts : list Type, functors.MixVariantFunctor._functor
-  (dependent_type_functor_rec ts W) (predicates_hered.pred rmap) -> A ts -> B ts -> predicates_hered.pred rmap) :=
-  forall n ts w x y, approx n (b ts w x y) =
-  approx n (b ts (functors.MixVariantFunctor.fmap (dependent_type_functor_rec ts W) (approx n) (approx n) w) x y).
-
-Definition super_non_expansive_la {W} la := @super_non_expansive_list W (fun ts w rho => map (fun l => !! (locald_denote l rho)) (la ts w)).
-
-Definition super_non_expansive_lb {B W} lb := forall v : B, @super_non_expansive_list W (fun ts w rho => map (fun l => !! (locald_denote l rho)) (lb ts w v)).
-
-Import List.
-
-(* A is the type of the abstract data. T is the type quantified over in the postcondition.
-   W is the TypeTree of the witness for the rest of the function. *)
-(*Notation atomic_spec1 T W args tz la P a t lb b E :=
-  (mk_funspec (pair args tz) cc_default (atomic_spec_type W T)
-   (fun (ts: list Type) '(w, Q) =>
-     PROP ()
-     (LOCALx (map (fun l => l ts w) la)
-     (SEP (atomic_shift (a ts w) (⊤ ∖ E) ∅ (b ts w) Q; P ts w))))
-   (fun (ts: list Type) '(w, Q) => EX v : T,
-     PROP () (LOCALx (map (fun l => l ts w v) lb)
-     (SEP (Q v)))) _ _).*)
-
-Lemma atomic_spec_nonexpansive_pre' : forall {A T} {t : Inhabitant T} W P L G R S2 E SQ
-  (HP : @super_non_expansive_list W (fun ts a _ => map prop (P ts a)))
-  (HL: forall n ts x, L ts x = L ts (functors.MixVariantFunctor.fmap _ (compcert_rmaps.RML.R.approx n) (compcert_rmaps.RML.R.approx n) x))
-  (HG: @super_non_expansive_list W (fun ts a rho => map (fun Q0 => prop (locald_denote (gvars Q0) rho)) (G ts a)))
-  (HR : @super_non_expansive_list W (fun ts a _ => R ts a)),
-  super_non_expansive_a S2 ->
-  super_non_expansive_E E ->
-  super_non_expansive_b SQ ->
-  @args_super_non_expansive (atomic_spec_type W T)
-  (fun ts (_a : functors.MixVariantFunctor._functor (dependent_type_functor_rec ts W) mpred * (T -> mpred)) =>
-    let '(w, Q) := _a in
-    PROPx (P ts w) (PARAMSx (L ts w) (GLOBALSx (G ts w)
-     (SEPx (atomic_shift(A := A ts) (S2 ts w) (⊤ ∖ E ts w) ∅ (SQ ts w) Q :: R ts w))))).
-Proof.
-  intros.
-  hnf; intros.
-  etransitivity; [|etransitivity; [
-    apply (PROP_PARAMS_GLOBALS_SEP_args_super_non_expansive' (atomic_spec_type W T) (fun ts x => P ts (fst x)) (fun ts x => L ts (fst x)) (fun ts x => G ts (fst x)) (fun ts '(w, Q) => atomic_shift(A := A ts) (S2 ts w) (⊤ ∖ E ts w) ∅ (SQ ts w) Q :: R ts w))|]].
-  - instantiate (9 := x). destruct x. reflexivity.
-  - intros ? ? (?, ?) ?; apply HP; auto.
-  - intros ? ? (?, ?); apply HL; auto.
-  - intros ? ? (?, ?); apply HG; auto.
-  - intros ? ? (?, ?) ?; constructor; [|apply HR; auto].
-    rewrite -> atomic_shift_nonexpansive by auto; setoid_rewrite atomic_shift_nonexpansive at 2; auto.
-    f_equal; f_equal; repeat extensionality; simpl.
-    + apply H.
-    + erewrite H0; reflexivity.
-    + apply H1.
-    + rewrite approx_idem; auto.
-  - destruct x as (?, ?); reflexivity.
-Qed.
-
 Definition atomic_spec_type0 W := ProdType W Mpred.
 
-Lemma atomic_spec_nonexpansive_pre0 : forall {A} W P L G R S2 E SQ
-  (HP : super_non_expansive_list (fun ts w _ => map prop (P ts w)))
-  (HL: forall n ts x, L ts x = L ts (functors.MixVariantFunctor.fmap _ (compcert_rmaps.RML.R.approx n) (compcert_rmaps.RML.R.approx n) x))
-  (HG: @super_non_expansive_list W (fun ts a rho => map (fun Q0 => prop (locald_denote (gvars Q0) rho)) (G ts a)))
-  (HR : super_non_expansive_list (fun ts w _ => R ts w)),
-  super_non_expansive_a S2 ->
-  super_non_expansive_E E ->
-  super_non_expansive_b SQ ->
-  @args_super_non_expansive (atomic_spec_type0 W)
-  (fun ts (_a : functors.MixVariantFunctor._functor (dependent_type_functor_rec ts W) mpred * mpred) =>
-    let '(w, Q) := _a in
-    PROPx (P ts w) (PARAMSx (L ts w) (GLOBALSx (G ts w)
-     (SEPx (atomic_shift(A := A ts)(B := unit) (S2 ts w) (⊤ ∖ E ts w) ∅ (SQ ts w) (fun _ => Q) :: R ts w))))).
-Proof.
-  intros.
-  hnf; intros.
-  etransitivity; [|etransitivity; [
-    apply (PROP_PARAMS_GLOBALS_SEP_args_super_non_expansive' (atomic_spec_type0 W) (fun ts x => P ts (fst x)) (fun ts x => L ts (fst x)) (fun ts x => G ts (fst x)) (fun ts '(w, Q) => atomic_shift(A := A ts) (S2 ts w) (⊤ ∖ E ts w) ∅ (SQ ts w) (fun _ => Q) :: R ts w))|]].
-  - instantiate (9 := x). destruct x. reflexivity.
-  - intros ? ? (?, ?) ?; apply HP; auto.
-  - intros ? ? (?, ?); apply HL; auto.
-  - intros ? ? (?, ?); apply HG; auto.
-  - intros ? ? (?, ?) ?; constructor; [|apply HR; auto].
-    rewrite -> atomic_shift_nonexpansive by auto; setoid_rewrite atomic_shift_nonexpansive at 2; auto.
-    f_equal; f_equal; repeat extensionality; simpl.
-    + apply H.
-    + erewrite H0; reflexivity.
-    + apply H1.
-    + rewrite approx_idem; auto.
-  - destruct x as (?, ?); reflexivity.
-Qed.
-
-Lemma atomic_spec_nonexpansive_pre : forall {A T} {t : Inhabitant T} W P L G R S2 E SQ Pre
-  (Heq : (forall ts (_a : functors.MixVariantFunctor._functor (dependent_type_functor_rec ts W) mpred * (T -> mpred)),
-   Pre ts _a = let '(w, Q) := _a in
-    PROPx (P ts w) (PARAMSx (L ts w) (GLOBALSx (G ts w)
-     (SEPx (atomic_shift(A := A ts) (S2 ts w) (⊤ ∖ E ts w) ∅ (SQ ts w) Q :: R ts w))))))
-  (HP : super_non_expansive_list (fun ts w _ => map prop (P ts w)))
-  (HL: forall n ts x, L ts x = L ts (functors.MixVariantFunctor.fmap _ (compcert_rmaps.RML.R.approx n) (compcert_rmaps.RML.R.approx n) x))
-  (HG: @super_non_expansive_list W (fun ts a rho => map (fun Q0 => prop (locald_denote (gvars Q0) rho)) (G ts a)))
-  (HR : super_non_expansive_list (fun ts w _ => R ts w)),
-  super_non_expansive_a S2 ->
-  super_non_expansive_E E ->
-  super_non_expansive_b SQ ->
-  @args_super_non_expansive (atomic_spec_type W T) Pre.
-Proof.
-  intros.
-  evar (Pre' : forall ts : list Type, functors.MixVariantFunctor._functor (dependent_type_functor_rec ts W) mpred * (T -> mpred) -> argsEnviron -> mpred).
-  replace Pre with Pre'; subst Pre'; [apply (atomic_spec_nonexpansive_pre'(A := A)); eauto|].
-  extensionality ts x; auto.
-Qed.
-
-Lemma atomic_spec_nonexpansive_post' : forall {T} W L R
-  (HL : forall v, super_non_expansive_list (fun ts w rho => map (fun l => !! (locald_denote l rho)) (L ts w v)))
-  (HR : forall v, super_non_expansive_list ((fun ts w _ => R ts w v))),
-  @super_non_expansive (atomic_spec_type W T)
-  (fun ts (_a : functors.MixVariantFunctor._functor (dependent_type_functor_rec ts W) mpred * (T -> mpred)) =>
-    let '(w, Q) := _a in
-    EX v : T,
-    PROP () (LOCALx (L ts w v) (SEPx (Q v :: R ts w v)))).
-Proof.
-  intros.
-  hnf; intros.
-  destruct x as (w, Q).
-  rewrite !approx_exp; f_equal; extensionality v.
-  etransitivity; [|etransitivity; [
-    apply (PROP_LOCAL_SEP_super_non_expansive' (atomic_spec_type W T) (fun ts '(w, _) => []) (fun ts '(w, _) => L ts w v) (fun ts '(w, Q) => Q v :: R ts w v))|]].
-  - instantiate (1 := rho); instantiate (1 := ts); instantiate (1 := (w, Q)); reflexivity.
-  - intros ? ? (?, ?) ?; constructor.
-  - intros ? ? (?, ?) ?; apply HL; auto.
-  - intros ? ? (?, ?) ?; constructor; [|apply HR; auto].
-    simpl; rewrite approx_idem; auto.
-  - reflexivity.
-Qed.
-
-Lemma atomic_spec_nonexpansive_post0 : forall W L R
-  (HL : super_non_expansive_list (fun ts w rho => map (fun l => !! (locald_denote l rho)) (L ts w)))
-  (HR : super_non_expansive_list ((fun ts w _ => R ts w))),
-  @super_non_expansive (atomic_spec_type0 W)
-  (fun ts (_a : functors.MixVariantFunctor._functor (dependent_type_functor_rec ts W) mpred * mpred) =>
-    let '(w, Q) := _a in
-    PROP () (LOCALx (L ts w) (SEPx (Q :: R ts w)))).
-Proof.
-  intros.
-  hnf; intros.
-  etransitivity; [|etransitivity; [
-    apply (PROP_LOCAL_SEP_super_non_expansive' (atomic_spec_type0 W) (fun ts '(w, _) => []) (fun ts '(w, _) => L ts w) (fun ts '(w, Q) => Q :: R ts w))|]].
-  - instantiate (1 := rho); instantiate (1 := ts); instantiate (1 := x); destruct x as (?, ?); reflexivity.
-  - intros ? ? (?, ?) ?; constructor.
-  - intros ? ? (?, ?) ?; apply HL; auto.
-  - intros ? ? (?, ?) ?; constructor; [|apply HR; auto].
-    simpl; rewrite approx_idem; auto.
-  - reflexivity.
-Qed.
-
-Lemma atomic_spec_nonexpansive_post : forall {T} W L R Post
-  (Heq : (forall ts (_a : functors.MixVariantFunctor._functor (dependent_type_functor_rec ts W) mpred * (T -> mpred)),
-  Post ts _a = let '(w, Q) := _a in
-    EX v : T,
-    PROP () (LOCALx (L ts w v) (SEPx (Q v :: R ts w v)))))
-  (HL : forall v, super_non_expansive_list (fun ts w rho => map (fun l => !! (locald_denote l rho)) (L ts w v)))
-  (HR : forall v, super_non_expansive_list ((fun ts w _ => R ts w v))),
-  @super_non_expansive (atomic_spec_type W T) Post.
-Proof.
-  intros.
-  evar (Post' : forall ts : list Type, functors.MixVariantFunctor._functor (dependent_type_functor_rec ts W) mpred * (T -> mpred) -> environ -> mpred).
-  replace Post with Post'; subst Post'; [apply atomic_spec_nonexpansive_post'; eauto|].
-  extensionality ts x; auto.
-Qed.
-
 (* A is the type of the abstract data. T is the type quantified over in the postcondition.
    W is the TypeTree of the witness for the rest of the function. *)
-Program Definition atomic_spec {A T} {t : Inhabitant T} W args tz la P G Qp a lb
-        b E
-   (HP : super_non_expansive' P) (HQp : forall v:T, super_non_expansive' (Qp v))
+Program Definition atomic_spec `{!VSTGS OK_ty Σ} {A T} {t : Inhabitant T} W args (tz : type)
+  (la : dtfr W -n> list.listO (leibnizO val)) (P : dtfr W -n> mpred) (G : dtfr W -n> leibnizO (list globals))
+  (Qp : T -> dtfr W -n> mpred) (a : dtfr W -n> _) (lb : dtfr W -n> T -d> leibnizO (list localdef))
+        (b : dtfr W -n> _) (E : dtfr W -n> leibnizO coPset)
+   (*(HP : super_non_expansive' P) (HQp : forall v:T, super_non_expansive' (Qp v))
   (Ha : super_non_expansive_a(A := A) a) (Hla: forall n ts x, la ts x = la ts (functors.MixVariantFunctor.fmap _ (compcert_rmaps.RML.R.approx n) (compcert_rmaps.RML.R.approx n) x))
   (HG: @super_non_expansive_list W (fun ts a rho => map (fun Q0 => prop (locald_denote (gvars Q0) rho)) (G ts a)))
   (HE: super_non_expansive_E E)
-  (Hlb : super_non_expansive_lb lb) (Hb : super_non_expansive_b b) :=
-  mk_funspec (pair args tz) cc_default (atomic_spec_type W T)
-  (fun (ts: list Type) '(w, Q) =>
+  (Hlb : super_non_expansive_lb lb) (Hb : super_non_expansive_b b)*) :=
+  mk_funspec(PROP1 := iProp Σ) (pair args tz) cc_default coPset_top (atomic_spec_type W T)
+  (λne '(w, Q),
     PROP ()
-    (PARAMSx (la ts w) (GLOBALSx (G ts w) (
-    (SEP (atomic_shift (a ts w) (⊤ ∖ E ts w) ∅ (b ts w) Q; P ts w))%assert5))))
-  (fun (ts: list Type) '(w, Q) => EX v : T,
-    PROP () (LOCALx (lb ts w v)
-    (SEP (Q v; Qp v ts w))%assert5)) _ _.
+    (PARAMSx (la w) (GLOBALSx (G w) (
+    (SEP (atomic_shift(A := A) (a w) (⊤ ∖ E w) ∅ (b w) Q; P w))%assert5))))
+  (λne '(w, Q), ∃ v : T,
+    PROP () (LOCALx (lb w v)
+    (SEP (Q v; Qp v w))%assert5)).
 Next Obligation.
 Proof.
-  intros; eapply atomic_spec_nonexpansive_pre; try eassumption.
-  { intros ? (?, ?). reflexivity. }
-  all: auto.
-  - constructor.
-  - repeat constructor; repeat intro; auto.
+  intros; intros (w1 & Q1) (w2 & Q2) (Hw & HQ) ?; simpl in *.
+  assert (la w1 = la w2) as ->.
+  { apply leibniz_equiv, (discrete_iff n); rewrite ?Hw //. apply _. }
+  assert (G w1 = G w2) as ->.
+  { apply leibniz_equiv, (discrete_iff n); rewrite ?Hw //. apply _. }
+  assert (E w1 = E w2) as ->.
+  { apply leibniz_equiv, (discrete_iff n); rewrite ?Hw //. apply _. }
+  solve_proper.
 Qed.
 Next Obligation.
 Proof.
-  intros; eapply atomic_spec_nonexpansive_post.
-  { intros ? (?, ?); reflexivity. }
-  - auto.
-  - repeat constructor.
-    unfold super_non_expansive, super_non_expansive' in *.
-    intros; apply HQp.
+  intros; intros (w1 & Q1) (w2 & Q2) (Hw & HQ) ?; simpl in *.
+  do 2 f_equiv.
+  intros v.
+  assert (lb w1 v = lb w2 v) as ->.
+  { assert (lb w1 ≡{n}≡ lb w2) as H by rewrite Hw //; apply H. }
+  solve_proper.
 Qed.
 
-(*Definition stable_spec_type W := ProdType (ProdType W
-  (ArrowType (DependentType 0) (ArrowType (DependentType 1) Mpred))) (ArrowType (DependentType 1) Mpred).
-
-Lemma stabilize : forall T W args tz P1 P2 Q1 Q2 neP1 neP2 neQ1 neQ2
-  PP la P a lb b Eo Ei Q'
-  (Hpre1 : forall ts w Q, P1 ts (w, Q) =
-     PROP (PP ts w)
-     (LOCALx (map (fun l => l ts w) la)
-     (SEP (atomic_shift (a ts w) Eo Ei (b ts w) Q; P ts w))))
-  (Hpost1 : forall ts w Q inv_names, Q1 ts (w, Q) =
-     EX v : T, PROP () (LOCALx (map (fun l => l ts w v) lb) (SEP (Q v))))
-  (Hpre2 : forall ts w b' Q, P2 ts (w, b', Q) =
-     PROP (PP ts w)
-     (LOCALx (map (fun l => l ts w) la)
-     (SEP (atomic_shift (a ts w) Eo Ei b' Q; P ts w))))
-  (Hpost2 : forall ts w b' Q, Q2 ts (w, b', Q) =
-    EX v1 : _, EX v2 : _,
-     PROP () (LOCALx (map (fun l => l ts w v2) lb)
-     (SEP (atomic_shift (a ts w) Eo Ei b' Q; Q' ts w v1 v2))))
-  (Hb : forall ts w v1 v2, b ts w v1 v2 |-- a ts w v1 * Q' ts w v1 v2),
-  funspec_sub (mk_funspec (pair args tz) cc_default (atomic_spec_type W T) P1 Q1 neP1 neQ1)
-    (mk_funspec (pair args tz) cc_default (stable_spec_type W) P2 Q2 neP2 neQ2).
-Proof.
-  intros; apply subsume_subsume.
-  unfold funspec_sub'; repeat (split; auto); intros.
-  destruct x2 as ((w, b'), Q).
-  simpl funsig_of_funspec.
-  rewrite Hpre2.
-  set (AS := atomic_shift _ _ _ _ _).
-  eapply derives_trans, ghost_seplog.bupd_intro.
-  Exists ts2 (w, (fun v2 => AS * EX v1 : _, Q' ts2 w v1 v2)) emp.
-  simpl in *; intro.
-  unfold liftx; simpl.
-  unfold lift.
-  rewrite emp_sepcon.
-  apply andp_right.
-  - apply andp_left2.
-    rewrite Hpre1.
-    unfold PROPx, LOCALx, SEPx; simpl.
-    do 2 (apply andp_derives; auto).
-    unfold AS, atomic_shift; Intros P'; Exists P'; cancel.
-    sep_apply cored_dup_cored.
-    apply andp_derives; auto.
-    iIntros "[H AS] P"; iMod ("H" with "P") as (v1) "[a H]".
-    iExists v1; iFrame.
-    iIntros "!>"; iSplit.
-    + iIntros "a".
-      iDestruct "AS" as "[_ e]"; iMod (cored_emp with "e") as "_".
-      iApply "H"; auto.
-    + iIntros (y) "b".
-      iDestruct (Hb with "b") as "[a Q]".
-      iMod ("H" with "a").
-      iIntros "!>"; iSplitR "Q".
-      * iExists P'; iFrame.
-      * iExists v1; auto.
-  - apply prop_right; intros.
-    apply andp_left2; rewrite emp_sepcon; auto.
-    rewrite Hpost1 Hpost2.
-    unfold PROPx, LOCALx, SEPx; simpl.
-    eapply derives_trans, ghost_seplog.bupd_intro.
-    Intros v2 v1; Exists v1 v2; rewrite sepcon_assoc; unfold AS; auto.
-Qed.
-
-Lemma stabilize0 : forall W args tz P1 P2 Q1 Q2 neP1 neP2 neQ1 neQ2
-  PP la P a lb b Eo Ei Q'
-  (Hpre1 : forall ts w Q, P1 ts (w, Q) =
-    PROP (PP ts w)
-     (LOCALx (map (fun l => l ts w) la)
-     (SEP (atomic_shift(B := unit) (a ts w) Eo Ei (b ts w) (fun _ => Q); P ts w))))
-  (Hpost1 : forall ts w Q, Q1 ts (w, Q) =
-     PROP () (LOCALx (map (fun l => l ts w) lb) ((SEPx (Q :: cons SPx%logic .. (cons SPy%logic nil) ..)))))
-  (Hpre2 : forall ts w b' Q, P2 ts (w, b', Q) =
-     PROP (PP ts w)
-     (LOCALx (map (fun l => l ts w) la)
-     (SEP (atomic_shift (a ts w) Eo Ei b' Q; P ts w))))
-  (Hpost2 : forall ts w b' Q inv_names, Q2 ts (w, b', Q) =
-    EX v1 : _,
-     PROP () (LOCALx (map (fun l => l ts w) lb)
-     (SEP (atomic_shift (a ts w) Eo Ei b' Q; Q' ts w v1))))
-  (Hb : forall ts w v1, b ts w v1 tt |-- a ts w v1 * Q' ts w v1),
-  funspec_sub (mk_funspec (pair args tz) cc_default (atomic_spec_type0 W) P1 Q1 neP1 neQ1)
-    (mk_funspec (pair args tz) cc_default (stable_spec_type W) P2 Q2 neP2 neQ2).
-Proof.
-  intros; apply subsume_subsume.
-  unfold funspec_sub'; repeat (split; auto); intros.
-  destruct x2 as ((w, b'), Q).
-  simpl funsig_of_funspec.
-  rewrite Hpre2.
-  set (AS := atomic_shift _ _ _ _ _).
-  eapply derives_trans, ghost_seplog.bupd_intro.
-  Exists ts2 (w, (AS * EX v1 : _, Q' ts2 w v1)) emp.
-  simpl in *; intro.
-  unfold liftx; simpl.
-  unfold lift.
-  rewrite emp_sepcon.
-  apply andp_right.
-  - apply andp_left2.
-    rewrite Hpre1.
-    unfold PROPx, LOCALx, SEPx; simpl.
-    do 2 (apply andp_derives; auto).
-    unfold AS, atomic_shift; Intros P'; Exists P'; cancel.
-    sep_apply cored_dup_cored.
-    apply andp_derives; auto.
-    iIntros "[H AS] P"; iMod ("H" with "P") as (v1) "[a H]".
-    iExists v1; iFrame.
-    iIntros "!>"; iSplit.
-    + iIntros "a".
-      iDestruct "AS" as "[_ e]"; iMod (cored_emp with "e") as "_".
-      iApply "H"; auto.
-    + iIntros ([]) "b".
-      iDestruct (Hb with "b") as "[a Q]".
-      iMod ("H" with "a").
-      iIntros "!>"; iSplitR "Q".
-      * iExists P'; iFrame.
-      * iExists v1; auto.
-  - apply prop_right; intros.
-    apply andp_left2; rewrite emp_sepcon; auto.
-    rewrite Hpost1 Hpost2.
-    unfold PROPx, LOCALx, SEPx; simpl.
-    eapply derives_trans, ghost_seplog.bupd_intro.
-    Intros v1; Exists v1; rewrite sepcon_assoc; unfold AS; auto.
-Qed.*)
-
-Require Import stdpp.hlist.
+Inductive tlist := tnil : tlist | tcons : ofe → tlist → tlist.
 
 (* Adapted from personal correspondence with Jason Gross, this lets us manipulate tuple types like they were lists. *)
-Fixpoint tuple_type (A : tlist) : Type :=
+Fixpoint tuple_type (A : tlist) : ofe :=
   match A with
   | tnil => unit
-  | tcons A As => A * tuple_type As
+  | tcons A As => prodO A (tuple_type As)
   end.
-Definition tcurry {A As B} (f : A -> tuple_type As -> B)
-  : tuple_type (tcons A As) -> B
-  := fun '(a, b) => f a b.
+Program Definition tcurry {A As B} (f : A -n> tuple_type As -n> B)
+  : tuple_type (tcons A As) -n> B
+  := λne '(a, b), f a b.
+Next Obligation.
+Proof.
+  intros; simpl.
+  intros (?, ?) (?, ?) (? & ?).
+  solve_proper.
+Qed.
 
-Fixpoint tuple_type_rev' (A : tlist) (acc : Type) : Type
+Fixpoint tuple_type_rev' (A : tlist) (acc : ofe) : ofe
   := match A with
      | tnil => acc
-     | tcons A As => tuple_type_rev' As (acc * A)
+     | tcons A As => tuple_type_rev' As (prodO acc A)
      end.
 
-Definition tuple_type_rev (A : tlist) : Type
+Definition tuple_type_rev (A : tlist) : ofe
   := match A with
      | tnil => unit
      | tcons A As => tuple_type_rev' As A
      end.
 
-Fixpoint tcurry_rev' (A : tlist) (acc : Type) {struct A}
-  : tuple_type_rev' A acc -> acc * tuple_type A
-  := match A return tuple_type_rev' A acc -> acc * tuple_type A with
-     | tnil => fun v => (v, tt)
-     | tcons A As => fun v => let '(sf, a, v) := tcurry_rev' As _ v in
+Program Fixpoint tcurry_rev' (A : tlist) (acc : ofe) {struct A}
+  : tuple_type_rev' A acc -n> prodO acc (tuple_type A)
+  := match A return tuple_type_rev' A acc -n> prodO acc (tuple_type A) with
+     | tnil => λne v, (v, tt)
+     | tcons A As => λne v, let '(sf, a, v) := tcurry_rev' As _ v in
                               (sf, (a, v))
      end.
-Definition tcurry_rev (A : tlist) : tuple_type_rev A -> tuple_type A
+Next Obligation.
+Proof. solve_proper. Qed.
+Next Obligation.
+Proof.
+  intros; simpl.
+  intros ???; simpl.
+  destruct (tcurry_rev' _ _ _) as ((x1, x2), x3) eqn: Hrevx.
+  destruct (tcurry_rev' _ _ y) as ((y1, y2), y3) eqn: Hrevy.
+  assert ((x1, x2, x3) ≡{n}≡ (y1, y2, y3)) as ((? & ?) & ?); last solve_proper.
+  rewrite -Hrevx -Hrevy H //.
+Defined.
+
+Program Definition tcurry_rev (A : tlist) : tuple_type_rev A -n> tuple_type A
   := match A with
-     | tnil => fun v => v
-     | tcons A As => fun v => tcurry_rev' As A v
+     | tnil => λne v, v
+     | tcons A As => λne v, tcurry_rev' As A v
      end.
+Next Obligation.
+Proof. solve_proper. Qed.
 
-Definition rev_curry {A B} (f : tuple_type A -> B) : tuple_type_rev A -> B
-  := fun v => f (tcurry_rev _ v).
+Program Definition rev_curry {A B} (f : tuple_type A -n> B) : tuple_type_rev A -n> B
+  := λne v, f (tcurry_rev _ v).
+Next Obligation.
+Proof. solve_proper. Qed.
 
-(* There must be a way to simplify this. *)
-Notation "'ATOMIC' 'TYPE' W 'OBJ' x : A 'INVS' E 'WITH' x1 , .. , xn 'PRE'  [ u , .. , v ] 'PROP' ( Px ; .. ; Py ) 'PARAMS' ( Lx ; .. ; Ly ) 'GLOBALS' ( Gx ; .. ; Gy ) 'SEP' ( S1x ; .. ; S1y ) '|' S2 'POST' [ tz ] 'EX' r : T , 'PROP' () 'LOCAL' ( LQx ; .. ; LQy ) 'SEP' ( SPx ; .. ; SPy ) '|' ( SQx ; .. ; SQy )" :=
-  (mk_funspec (pair (cons u%type .. (cons v%type nil) ..) tz) cc_default (atomic_spec_type W T)
-   (fun (ts: list Type) => rev_curry (tcurry (fun x1 => .. (tcurry (fun xn => tcurry (fun (Q : T -> mpred) (_ : tuple_type tnil) =>
+(* There must be a way to simplify this. Maybe telescopes? *)
+Notation "'ATOMIC' 'TYPE' W 'OBJ' x : A 'INVS' E 'WITH' x1 , .. , xn 'PRE'  [ u , .. , v ] 'PROP' ( Px ; .. ; Py ) 'PARAMS' ( Lx ; .. ; Ly ) 'GLOBALS' ( Gx ; .. ; Gy ) 'SEP' ( S1x ; .. ; S1y ) '|' S2 'POST' [ tz ] '∃' r : T , 'PROP' () 'LOCAL' ( LQx ; .. ; LQy ) 'SEP' ( SPx ; .. ; SPy ) '|' ( SQx ; .. ; SQy )" :=
+  (mk_funspec (pair (cons u%type .. (cons v%type nil) ..) tz) cc_default ⊤ (atomic_spec_type W T)
+   (rev_curry (tcurry (λne x1, .. (tcurry (λne xn, tcurry (λne (Q : T -> mpred) (_ : tuple_type tnil),
      PROPx (cons Px%type .. (cons Py%type nil) ..)
      (PARAMSx (cons Lx%type .. (cons Ly%type nil) ..) (GLOBALSx (cons Gx .. (cons Gy nil) ..)
-     (SEPx (cons (atomic_shift (fun x => S2) (⊤ ∖ E) ∅ (fun x r => fold_right_sepcon (cons SQx%logic .. (cons SQy%logic nil) ..)) Q) (cons S1x%logic .. (cons S1y%logic nil) ..)))))))) ..)))
-   (fun (ts: list Type) => rev_curry (tcurry (fun x1 => .. (tcurry (fun xn => tcurry (fun (Q : T -> mpred) (_ : tuple_type tnil) =>
-    @exp (environ -> mpred) _ T (fun r =>
+     (SEPx (cons (atomic_shift (fun x => S2) (⊤ ∖ E) ∅ (fun x r => fold_right_sepcon (cons SQx%I .. (cons SQy%I nil) ..)) Q) (cons S1x%I .. (cons S1y%I nil) ..)))))))) ..)))
+   (rev_curry (tcurry (λne x1, .. (tcurry (λne xn, tcurry (λne (Q : T -> mpred) (_ : tuple_type tnil),
+    bi_exist(A := T) (fun r =>
      PROP () (LOCALx (cons LQx .. (cons LQy nil) ..) ((SEPx (Q r :: cons SPx .. (cons SPy nil) ..)))))))) ..)))
-   (@atomic_spec_nonexpansive_pre' (fun _ => A) T _ W
-      (fun (ts: list Type) => rev_curry (tcurry (fun x1 => .. (tcurry (fun xn (_ : tuple_type tnil) => (cons Px%type .. (cons Py%type nil) ..))) ..)))
-      (fun (ts: list Type) => rev_curry (tcurry (fun x1 => .. (tcurry (fun xn (_ : tuple_type tnil) => (cons Lx%type .. (cons Ly%type nil) ..))) ..)))
-      (fun (ts: list Type) => rev_curry (tcurry (fun x1 => .. (tcurry (fun xn (_ : tuple_type tnil) => (cons Gx .. (cons Gy nil) ..))) ..)))
-      (fun (ts: list Type) => rev_curry (tcurry (fun x1 => .. (tcurry (fun xn (_ : tuple_type tnil) => (cons S1x%logic .. (cons S1y%logic nil) ..))) ..)))
-      (fun (ts: list Type) => rev_curry (tcurry (fun x1 => .. (tcurry (fun xn (_ : tuple_type tnil) x => S2)) ..)))
-      (fun (ts: list Type) => rev_curry (tcurry (fun x1 => .. (tcurry (fun xn (_ : tuple_type tnil) => E)) ..)))
-      (fun (ts: list Type) => rev_curry (tcurry (fun x1 => .. (tcurry (fun xn (_ : tuple_type tnil) x r => fold_right_sepcon (cons SQx%logic .. (cons SQy%logic nil) ..))) ..)))
-     _ _ _ _ _ _ _)
-  (atomic_spec_nonexpansive_post' W
-      (fun (ts: list Type) => rev_curry (tcurry (fun x1 => .. (tcurry (fun xn (_ : tuple_type tnil) r => (cons LQx%assert3 .. (cons LQy%assert3 nil) ..))) ..)))
-      (fun (ts: list Type) => rev_curry (tcurry (fun x1 => .. (tcurry (fun xn (_ : tuple_type tnil) r => (cons SPx%assert3 .. (cons SPy%assert3 nil) ..))) ..))) _ _))
+   )
   (at level 200, x1 closed binder, xn closed binder, x at level 0, E at level 0, S2 at level 0, r at level 0, T at level 0).
 
-Notation "'ATOMIC' 'TYPE' W 'OBJ' x 'INVS' E 'WITH' x1 , .. , xn 'PRE'  [ u , .. , v ] 'PROP' ( Px ; .. ; Py ) 'PARAMS' ( Lx ; .. ; Ly ) 'GLOBALS' ( Gx ; .. ; Gy ) 'SEP' ( S1x ; .. ; S1y ) '|' S2 'POST' [ tz ] 'EX' r : T , 'PROP' () 'LOCAL' ( LQx ; .. ; LQy ) 'SEP' ( SPx ; .. ; SPy ) '|' ( SQx ; .. ; SQy )" :=
-  (mk_funspec (pair (cons u%type .. (cons v%type nil) ..) tz) cc_default (atomic_spec_type W T)
-   (fun (ts: list Type) => rev_curry (tcurry (fun x1 => .. (tcurry (fun xn => tcurry (fun (Q : T -> mpred) (_ : tuple_type tnil) =>
+Notation "'ATOMIC' 'TYPE' W 'OBJ' x 'INVS' E 'WITH' x1 , .. , xn 'PRE'  [ u , .. , v ] 'PROP' ( Px ; .. ; Py ) 'PARAMS' ( Lx ; .. ; Ly ) 'GLOBALS' ( Gx ; .. ; Gy ) 'SEP' ( S1x ; .. ; S1y ) '|' S2 'POST' [ tz ] '∃' r : T , 'PROP' () 'LOCAL' ( LQx ; .. ; LQy ) 'SEP' ( SPx ; .. ; SPy ) '|' ( SQx ; .. ; SQy )" :=
+  (mk_funspec (pair (cons u%type .. (cons v%type nil) ..) tz) cc_default ⊤ (atomic_spec_type W T)
+   (rev_curry (tcurry (λne x1, .. (tcurry (λne xn, tcurry (λne (Q : T -> mpred) (_ : tuple_type tnil),
      PROPx (cons Px%type .. (cons Py%type nil) ..)
      (PARAMSx (cons Lx%type .. (cons Ly%type nil) ..) (GLOBALSx (cons Gx .. (cons Gy nil) ..)
-     (SEPx (cons (atomic_shift (fun x => S2) (⊤ ∖ E) ∅ (fun x r => fold_right_sepcon (cons SQx%logic .. (cons SQy%logic nil) ..)) Q) (cons S1x%logic .. (cons S1y%logic nil) ..)))))))) ..)))
-   (fun (ts: list Type) => rev_curry (tcurry (fun x1 => .. (tcurry (fun xn => tcurry (fun (Q : T -> mpred) (_ : tuple_type tnil) =>
-    @exp (environ -> mpred) _ T (fun r =>
+     (SEPx (cons (atomic_shift (fun x => S2) (⊤ ∖ E) ∅ (fun x r => fold_right_sepcon (cons SQx%I .. (cons SQy%I nil) ..)) Q) (cons S1x%I .. (cons S1y%I nil) ..)))))))) ..)))
+   (rev_curry (tcurry (λne x1, .. (tcurry (λne xn, tcurry (λne (Q : T -> mpred) (_ : tuple_type tnil),
+    bi_exist(A := T) (fun r =>
      PROP () (LOCALx (cons LQx .. (cons LQy nil) ..) ((SEPx (Q r :: cons SPx .. (cons SPy nil) ..)))))))) ..)))
-   (@atomic_spec_nonexpansive_pre' _ T _ W
-      (fun (ts: list Type) => rev_curry (tcurry (fun x1 => .. (tcurry (fun xn (_ : tuple_type tnil) => (cons Px%type .. (cons Py%type nil) ..))) ..)))
-      (fun (ts: list Type) => rev_curry (tcurry (fun x1 => .. (tcurry (fun xn (_ : tuple_type tnil) => (cons Lx%type .. (cons Ly%type nil) ..))) ..)))
-      (fun (ts: list Type) => rev_curry (tcurry (fun x1 => .. (tcurry (fun xn (_ : tuple_type tnil) => (cons Gx .. (cons Gy nil) ..))) ..)))
-      (fun (ts: list Type) => rev_curry (tcurry (fun x1 => .. (tcurry (fun xn (_ : tuple_type tnil) => (cons S1x%logic .. (cons S1y%logic nil) ..))) ..)))
-      (fun (ts: list Type) => rev_curry (tcurry (fun x1 => .. (tcurry (fun xn (_ : tuple_type tnil) x => S2)) ..)))       (fun (ts: list Type) => rev_curry (tcurry (fun x1 => .. (tcurry (fun xn (_ : tuple_type tnil) => E)) ..)))
-      (fun (ts: list Type) => rev_curry (tcurry (fun x1 => .. (tcurry (fun xn (_ : tuple_type tnil) x r => fold_right_sepcon (cons SQx%logic .. (cons SQy%logic nil) ..))) ..)))
-     _ _ _ _ _ _ _)
-  (atomic_spec_nonexpansive_post' W
-      (fun (ts: list Type) => rev_curry (tcurry (fun x1 => .. (tcurry (fun xn (_ : tuple_type tnil) r => (cons LQx%assert3 .. (cons LQy%assert3 nil) ..))) ..)))
-      (fun (ts: list Type) => rev_curry (tcurry (fun x1 => .. (tcurry (fun xn (_ : tuple_type tnil) r => (cons SPx%assert3 .. (cons SPy%assert3 nil) ..))) ..))) _ _))
+   )
   (at level 200, x1 closed binder, xn closed binder, x at level 0, E at level 0, S2 at level 0, r at level 0, T at level 0).
 
-Notation "'ATOMIC' 'TYPE' W 'OBJ' x 'INVS' E 'WITH' x1 , .. , xn 'PRE'  [ u , .. , v ] 'PROP' ( Px ; .. ; Py ) 'PARAMS' ( Lx ; .. ; Ly ) 'GLOBALS' ( Gx ; .. ; Gy ) 'SEP' ( S1x ; .. ; S1y ) '|' S2 'POST' [ tz ] 'EX' r : T , 'PROP' () 'LOCAL' () 'SEP' ( SPx ; .. ; SPy ) '|' ( SQx ; .. ; SQy )" :=
-  (mk_funspec (pair (cons u%type .. (cons v%type nil) ..) tz) cc_default (atomic_spec_type W T)
-   (fun (ts: list Type) => rev_curry (tcurry (fun x1 => .. (tcurry (fun xn => tcurry (fun (Q : T -> mpred) (_ : tuple_type tnil) =>
+Notation "'ATOMIC' 'TYPE' W 'OBJ' x 'INVS' E 'WITH' x1 , .. , xn 'PRE'  [ u , .. , v ] 'PROP' ( Px ; .. ; Py ) 'PARAMS' ( Lx ; .. ; Ly ) 'GLOBALS' ( Gx ; .. ; Gy ) 'SEP' ( S1x ; .. ; S1y ) '|' S2 'POST' [ tz ] '∃' r : T , 'PROP' () 'LOCAL' () 'SEP' ( SPx ; .. ; SPy ) '|' ( SQx ; .. ; SQy )" :=
+  (mk_funspec (pair (cons u%type .. (cons v%type nil) ..) tz) cc_default ⊤ (atomic_spec_type W T)
+   (rev_curry (tcurry (λne x1, .. (tcurry (λne xn, tcurry (λne (Q : T -> mpred) (_ : tuple_type tnil),
      PROPx (cons Px%type .. (cons Py%type nil) ..)
      (PARAMSx (cons Lx%type .. (cons Ly%type nil) ..) (GLOBALSx (cons Gx .. (cons Gy nil) ..)
-     (SEPx (cons (atomic_shift (fun x => S2) (⊤ ∖ E) ∅ (fun x r => fold_right_sepcon (cons SQx%logic .. (cons SQy%logic nil) ..)) Q) (cons S1x%logic .. (cons S1y%logic nil) ..)))))))) ..)))
-   (fun (ts: list Type) => rev_curry (tcurry (fun x1 => .. (tcurry (fun xn => tcurry (fun (Q : T -> mpred) (_ : tuple_type tnil) =>
-    @exp (environ -> mpred) _ T (fun r =>
+     (SEPx (cons (atomic_shift (fun x => S2) (⊤ ∖ E) ∅ (fun x r => fold_right_sepcon (cons SQx%I .. (cons SQy%I nil) ..)) Q) (cons S1x%I .. (cons S1y%I nil) ..)))))))) ..)))
+   (rev_curry (tcurry (λne x1, .. (tcurry (λne xn, tcurry (λne (Q : T -> mpred) (_ : tuple_type tnil),
+    bi_exist(A := T) (fun r =>
      PROP () (LOCAL () (SEPx (Q r :: cons SPx .. (cons SPy nil) ..))))))) ..)))
-   (@atomic_spec_nonexpansive_pre' _ T _ W
-      (fun (ts: list Type) => rev_curry (tcurry (fun x1 => .. (tcurry (fun xn (_ : tuple_type tnil) => (cons Px%type .. (cons Py%type nil) ..))) ..)))
-      (fun (ts: list Type) => rev_curry (tcurry (fun x1 => .. (tcurry (fun xn (_ : tuple_type tnil) => (cons Lx%type .. (cons Ly%type nil) ..))) ..)))
-      (fun (ts: list Type) => rev_curry (tcurry (fun x1 => .. (tcurry (fun xn (_ : tuple_type tnil) => (cons Gx .. (cons Gy nil) ..))) ..)))
-      (fun (ts: list Type) => rev_curry (tcurry (fun x1 => .. (tcurry (fun xn (_ : tuple_type tnil) => (cons S1x%logic .. (cons S1y%logic nil) ..))) ..)))
-      (fun (ts: list Type) => rev_curry (tcurry (fun x1 => .. (tcurry (fun xn (_ : tuple_type tnil) x => S2)) ..)))       (fun (ts: list Type) => rev_curry (tcurry (fun x1 => .. (tcurry (fun xn (_ : tuple_type tnil) => E)) ..)))
-      (fun (ts: list Type) => rev_curry (tcurry (fun x1 => .. (tcurry (fun xn (_ : tuple_type tnil) x r => fold_right_sepcon (cons SQx%logic .. (cons SQy%logic nil) ..))) ..)))
-     _ _ _ _ _ _ _)
-  (atomic_spec_nonexpansive_post' W
-      (fun (ts: list Type) => rev_curry (tcurry (fun x1 => .. (tcurry (fun xn (_ : tuple_type tnil) r => nil)) ..)))
-      (fun (ts: list Type) => rev_curry (tcurry (fun x1 => .. (tcurry (fun xn (_ : tuple_type tnil) r => (cons SPx%assert5%assert3 .. (cons SPy%assert5%assert3 nil) ..))) ..))) _ _))
+   )
   (at level 200, x1 closed binder, xn closed binder, x at level 0, E at level 0, S2 at level 0, r at level 0, T at level 0).
 
 Notation "'ATOMIC' 'TYPE' W 'OBJ' x 'INVS' E 'WITH' x1 , .. , xn 'PRE'  [ u , .. , v ] 'PROP' ( Px ; .. ; Py ) 'PARAMS' ( Lx ; .. ; Ly ) 'GLOBALS' ( Gx ; .. ; Gy ) 'SEP' ( S1x ; .. ; S1y ) '|' S2 'POST' [ tz ] 'PROP' () 'LOCAL' ( LQx ; .. ; LQy ) 'SEP' ( SPx ; .. ; SPy ) '|' ( SQx ; .. ; SQy )" :=
-  (mk_funspec (pair (cons u%type .. (cons v%type nil) ..) tz) cc_default (atomic_spec_type0 W)
-   (fun (ts: list Type) => rev_curry (tcurry (fun x1 => .. (tcurry (fun xn => tcurry (fun (Q : mpred) (_ : tuple_type tnil) =>
-     PROPx (cons Px%type .. (cons Py%type nil) ..)
+  (mk_funspec (pair (cons u%type .. (cons v%type nil) ..) tz) cc_default ⊤ (atomic_spec_type0 W)
+   (rev_curry (tcurry (λne x1, .. (tcurry (λne xn, tcurry (λne (Q : mpred) (_ : tuple_type tnil),  PROPx (cons Px%type .. (cons Py%type nil) ..)
      (PARAMSx (cons Lx%type .. (cons Ly%type nil) ..) (GLOBALSx (cons Gx .. (cons Gy nil) ..)
-     (SEPx (cons (atomic_shift(B := unit) (fun x => S2) (⊤ ∖ E) ∅ (fun x _ => fold_right_sepcon (cons SQx%logic .. (cons SQy%logic nil) ..)) (fun _ => Q)) (cons S1x%logic .. (cons S1y%logic nil) ..)))))))) ..)))
-   (fun (ts: list Type) => rev_curry (tcurry (fun x1 => .. (tcurry (fun xn => tcurry (fun (Q : mpred) (_ : tuple_type tnil) =>
-     PROP () (LOCALx (cons LQx .. (cons LQy nil) ..) (SEPx (Q :: cons SPx .. (cons SPy nil) ..)))))) ..)))
-   (@atomic_spec_nonexpansive_pre0 _ W
-      (fun (ts: list Type) => rev_curry (tcurry (fun x1 => .. (tcurry (fun xn (_ : tuple_type tnil) => (cons Px%type .. (cons Py%type nil) ..))) ..)))
-      (fun (ts: list Type) => rev_curry (tcurry (fun x1 => .. (tcurry (fun xn (_ : tuple_type tnil) => (cons Lx%type .. (cons Ly%type nil) ..))) ..)))
-      (fun (ts: list Type) => rev_curry (tcurry (fun x1 => .. (tcurry (fun xn (_ : tuple_type tnil) => (cons Gx .. (cons Gy nil) ..))) ..)))
-      (fun (ts: list Type) => rev_curry (tcurry (fun x1 => .. (tcurry (fun xn (_ : tuple_type tnil) => (cons S1x%logic .. (cons S1y%logic nil) ..))) ..)))
-      (fun (ts: list Type) => rev_curry (tcurry (fun x1 => .. (tcurry (fun xn (_ : tuple_type tnil) x => S2)) ..)))       (fun (ts: list Type) => rev_curry (tcurry (fun x1 => .. (tcurry (fun xn (_ : tuple_type tnil) => E)) ..)))
-      (fun (ts: list Type) => rev_curry (tcurry (fun x1 => .. (tcurry (fun xn (_ : tuple_type tnil) x _ => fold_right_sepcon (cons SQx%logic .. (cons SQy%logic nil) ..))) ..)))
-     _ _ _ _ _ _ _)
-  (atomic_spec_nonexpansive_post0 W
-      (fun (ts: list Type) => rev_curry (tcurry (fun x1 => .. (tcurry (fun xn (_ : tuple_type tnil) => (cons LQx%assert3 .. (cons LQy%assert3 nil) ..))) ..)))
-      (fun (ts: list Type) => rev_curry (tcurry (fun x1 => .. (tcurry (fun xn (_ : tuple_type tnil) => (cons SPx%assert3 .. (cons SPy%assert3 nil) ..))) ..))) _ _))
+     (SEPx (cons (atomic_shift(B := unit) (fun x => S2) (⊤ ∖ E) ∅ (fun x _ => fold_right_sepcon (cons SQx%I .. (cons SQy%I nil) ..)) (fun _ => Q)) (cons S1x%I .. (cons S1y%I nil) ..)))))))) ..)))
+   (rev_curry (tcurry (λne x1, .. (tcurry (λne xn, tcurry (λne (Q : mpred) (_ : tuple_type tnil),  PROP () (LOCALx (cons LQx .. (cons LQy nil) ..) (SEPx (Q :: cons SPx .. (cons SPy nil) ..)))))) ..)))
+   )
   (at level 200, x1 closed binder, xn closed binder, x at level 0, E at level 0, S2 at level 0).
 
 Notation "'ATOMIC' 'TYPE' W 'OBJ' x 'INVS' E 'WITH' x1 , .. , xn 'PRE'  [ u , .. , v ] 'PROP' ( Px ; .. ; Py ) 'PARAMS' ( Lx ; .. ; Ly ) 'GLOBALS' ( Gx ; .. ; Gy ) 'SEP' ( S1x ; .. ; S1y ) '|' S2 'POST' [ tz ] 'PROP' () 'LOCAL' () 'SEP' ( SPx ; .. ; SPy ) '|' ( SQx ; .. ; SQy )" :=
-  (mk_funspec (pair (cons u%type .. (cons v%type nil) ..) tz) cc_default (atomic_spec_type0 W)
-   (fun (ts: list Type) => rev_curry (tcurry (fun x1 => .. (tcurry (fun xn => tcurry (fun (Q : mpred) (_ : tuple_type tnil) =>
-     PROPx (cons Px%type .. (cons Py%type nil) ..)
+  (mk_funspec (pair (cons u%type .. (cons v%type nil) ..) tz) cc_default ⊤ (atomic_spec_type0 W)
+   (rev_curry (tcurry (λne x1, .. (tcurry (λne xn, tcurry (λne (Q : mpred) (_ : tuple_type tnil),  PROPx (cons Px%type .. (cons Py%type nil) ..)
      (PARAMSx (cons Lx%type .. (cons Ly%type nil) ..) (GLOBALSx (cons Gx .. (cons Gy nil) ..)
-     (SEPx (cons (atomic_shift(B := unit) (fun x => S2) (⊤ ∖ E) ∅ (fun x _ => fold_right_sepcon (cons SQx%logic .. (cons SQy%logic nil) ..)) (fun _ => Q)) (cons S1x%logic .. (cons S1y%logic nil) ..)))))))) ..)))
-   (fun (ts: list Type) => rev_curry (tcurry (fun x1 => .. (tcurry (fun xn => tcurry (fun (Q : mpred) (_ : tuple_type tnil) =>
-     PROP () LOCAL () (SEPx (Q :: cons SPx .. (cons SPy nil) ..))))) ..)))
-   (@atomic_spec_nonexpansive_pre0 _ W
-      (fun (ts: list Type) => rev_curry (tcurry (fun x1 => .. (tcurry (fun xn (_ : tuple_type tnil) => (cons Px%type .. (cons Py%type nil) ..))) ..)))
-      (fun (ts: list Type) => rev_curry (tcurry (fun x1 => .. (tcurry (fun xn (_ : tuple_type tnil) => (cons Lx%type .. (cons Ly%type nil) ..))) ..)))
-      (fun (ts: list Type) => rev_curry (tcurry (fun x1 => .. (tcurry (fun xn (_ : tuple_type tnil) => (cons Gx .. (cons Gy nil) ..))) ..)))
-      (fun (ts: list Type) => rev_curry (tcurry (fun x1 => .. (tcurry (fun xn (_ : tuple_type tnil) => (cons S1x%logic .. (cons S1y%logic nil) ..))) ..)))
-      (fun (ts: list Type) => rev_curry (tcurry (fun x1 => .. (tcurry (fun xn (_ : tuple_type tnil) x => S2)) ..)))       (fun (ts: list Type) => rev_curry (tcurry (fun x1 => .. (tcurry (fun xn (_ : tuple_type tnil) => E)) ..)))
-      (fun (ts: list Type) => rev_curry (tcurry (fun x1 => .. (tcurry (fun xn (_ : tuple_type tnil) x _ => fold_right_sepcon (cons SQx%logic .. (cons SQy%logic nil) ..))) ..)))
-     _ _ _ _ _ _ _)
-  (atomic_spec_nonexpansive_post0 W
-      (fun (ts: list Type) => rev_curry (tcurry (fun x1 => .. (tcurry (fun xn (_ : tuple_type tnil) => nil)) ..)))
-      (fun (ts: list Type) => rev_curry (tcurry (fun x1 => .. (tcurry (fun xn (_ : tuple_type tnil) => (cons SPx%assert5%assert3 .. (cons SPy%assert5%assert3 nil) ..))) ..))) _ _))
+     (SEPx (cons (atomic_shift(B := unit) (fun x => S2) (⊤ ∖ E) ∅ (fun x _ => fold_right_sepcon (cons SQx%I .. (cons SQy%I nil) ..)) (fun _ => Q)) (cons S1x%I .. (cons S1y%I nil) ..)))))))) ..)))
+   (rev_curry (tcurry (λne x1, .. (tcurry (λne xn, tcurry (λne (Q : mpred) (_ : tuple_type tnil),  PROP () LOCAL () (SEPx (Q :: cons SPx .. (cons SPy nil) ..))))) ..)))
+   )
   (at level 200, x1 closed binder, xn closed binder, x at level 0, E at level 0, S2 at level 0).
 
 Notation "'ATOMIC' 'TYPE' W 'INVS' E 'WITH' x1 , .. , xn 'PRE'  [ u , .. , v ] 'PROP' () 'PARAMS' ( Lx ; .. ; Ly ) 'SEP' () '|' S2 'POST' [ tz ] 'PROP' () 'LOCAL' () 'SEP' ( SPx ; .. ; SPy ) '|' ( SQx ; .. ; SQy )" :=
-  (mk_funspec (pair (cons u%type .. (cons v%type nil) ..) tz) cc_default (atomic_spec_type0 W)
-   (fun (ts: list Type) => rev_curry (tcurry (fun x1 => .. (tcurry (fun xn => tcurry (fun (Q : mpred) (_ : tuple_type tnil) =>
-     PROPx nil
+  (mk_funspec (pair (cons u%type .. (cons v%type nil) ..) tz) cc_default ⊤ (atomic_spec_type0 W)
+   (rev_curry (tcurry (λne x1, .. (tcurry (λne xn, tcurry (λne (Q : mpred) (_ : tuple_type tnil),  PROPx nil
      (PARAMSx (cons Lx%type .. (cons Ly%type nil) ..) (GLOBALSx nil
-     (SEPx (cons (atomic_shift(B := unit) (fun _ : unit => S2) (⊤ ∖ E) ∅ (fun (_ : unit) _ => fold_right_sepcon (cons SQx%logic .. (cons SQy%logic nil) ..)) (fun _ => Q)) nil))))))) ..)))
-   (fun (ts: list Type) => rev_curry (tcurry (fun x1 => .. (tcurry (fun xn => tcurry (fun (Q : mpred) (_ : tuple_type tnil) =>
-     PROP () LOCAL () (SEPx (Q :: cons SPx .. (cons SPy nil) ..))))) ..)))
-   (@atomic_spec_nonexpansive_pre0 _ W
-      (fun (ts: list Type) => rev_curry (tcurry (fun x1 => .. (tcurry (fun xn (_ : tuple_type tnil) => nil)) ..)))
-      (fun (ts: list Type) => rev_curry (tcurry (fun x1 => .. (tcurry (fun xn (_ : tuple_type tnil) => (cons Lx%type .. (cons Ly%type nil) ..))) ..)))
-      (fun (ts: list Type) => rev_curry (tcurry (fun x1 => .. (tcurry (fun xn (_ : tuple_type tnil) => nil)) ..)))
-      (fun (ts: list Type) => rev_curry (tcurry (fun x1 => .. (tcurry (fun xn (_ : tuple_type tnil) => nil)) ..)))
-      (fun (ts: list Type) => rev_curry (tcurry (fun x1 => .. (tcurry (fun xn (_ : tuple_type tnil) (_ : unit) => S2)) ..)))       (fun (ts: list Type) => rev_curry (tcurry (fun x1 => .. (tcurry (fun xn (_ : tuple_type tnil) => E)) ..)))
-      (fun (ts: list Type) => rev_curry (tcurry (fun x1 => .. (tcurry (fun xn (_ : tuple_type tnil) (_ : unit) _ => fold_right_sepcon (cons SQx%logic .. (cons SQy%logic nil) ..))) ..)))
-     _ _ _ _ _ _ _)
-  (atomic_spec_nonexpansive_post0 W
-      (fun (ts: list Type) => rev_curry (tcurry (fun x1 => .. (tcurry (fun xn (_ : tuple_type tnil) => nil)) ..)))
-      (fun (ts: list Type) => rev_curry (tcurry (fun x1 => .. (tcurry (fun xn (_ : tuple_type tnil) => (cons SPx%assert5%assert3 .. (cons SPy%assert5%assert3 nil) ..))) ..))) _ _))
+     (SEPx (cons (atomic_shift(B := unit) (fun _ : unit => S2) (⊤ ∖ E) ∅ (fun (_ : unit) _ => fold_right_sepcon (cons SQx%I .. (cons SQy%I nil) ..)) (fun _ => Q)) nil))))))) ..)))
+   (rev_curry (tcurry (λne x1, .. (tcurry (λne xn, tcurry (λne (Q : mpred) (_ : tuple_type tnil),  PROP () LOCAL () (SEPx (Q :: cons SPx .. (cons SPy nil) ..))))) ..)))
+   )
   (at level 200, x1 closed binder, xn closed binder, E at level 0, S2 at level 0).
 
 Notation "'ATOMIC' 'TYPE' W 'INVS' E 'WITH' x1 , .. , xn 'PRE'  [ u , .. , v ] 'PROP' () 'PARAMS' ( Lx ; .. ; Ly ) 'SEP' ( S1x ; .. ; S1y ) '|' S2 'POST' [ tz ] 'PROP' () 'LOCAL' () 'SEP' () '|' ( SQx ; .. ; SQy )" :=
-  (mk_funspec (pair (cons u%type .. (cons v%type nil) ..) tz) cc_default (atomic_spec_type0 W)
-   (fun (ts: list Type) => rev_curry (tcurry (fun x1 => .. (tcurry (fun xn => tcurry (fun (Q : mpred) (_ : tuple_type tnil) =>
-     PROPx nil
+  (mk_funspec (pair (cons u%type .. (cons v%type nil) ..) tz) cc_default ⊤ (atomic_spec_type0 W)
+   (rev_curry (tcurry (λne x1, .. (tcurry (λne xn, tcurry (λne (Q : mpred) (_ : tuple_type tnil),  PROPx nil
      (PARAMSx (cons Lx%type .. (cons Ly%type nil) ..) (GLOBALSx nil
-     (SEPx (cons (atomic_shift(B := unit) (fun (_ : unit) => S2) (⊤ ∖ E) ∅ (fun x _ => fold_right_sepcon (cons SQx%logic .. (cons SQy%logic nil) ..)) (fun _ => Q)) (cons S1x%logic .. (cons S1y%logic nil) ..)))))))) ..)))
-   (fun (ts: list Type) => rev_curry (tcurry (fun x1 => .. (tcurry (fun xn => tcurry (fun (Q : mpred) (_ : tuple_type tnil) =>
-     PROP () LOCAL () (SEPx (Q :: nil))))) ..)))
-   (@atomic_spec_nonexpansive_pre0 _ W
-      (fun (ts: list Type) => rev_curry (tcurry (fun x1 => .. (tcurry (fun xn (_ : tuple_type tnil) => nil)) ..)))
-      (fun (ts: list Type) => rev_curry (tcurry (fun x1 => .. (tcurry (fun xn (_ : tuple_type tnil) => (cons Lx%type .. (cons Ly%type nil) ..))) ..)))
-      (fun (ts: list Type) => rev_curry (tcurry (fun x1 => .. (tcurry (fun xn (_ : tuple_type tnil) => nil)) ..)))
-      (fun (ts: list Type) => rev_curry (tcurry (fun x1 => .. (tcurry (fun xn (_ : tuple_type tnil) => (cons S1x%logic .. (cons S1y%logic nil) ..))) ..)))
-      (fun (ts: list Type) => rev_curry (tcurry (fun x1 => .. (tcurry (fun xn (_ : tuple_type tnil) (_ : unit) => S2)) ..)))       (fun (ts: list Type) => rev_curry (tcurry (fun x1 => .. (tcurry (fun xn (_ : tuple_type tnil) => E)) ..)))
-      (fun (ts: list Type) => rev_curry (tcurry (fun x1 => .. (tcurry (fun xn (_ : tuple_type tnil) (_ : unit) _ => fold_right_sepcon (cons SQx%logic .. (cons SQy%logic nil) ..))) ..)))
-     _ _ _ _ _ _ _)
-  (atomic_spec_nonexpansive_post0 W
-      (fun (ts: list Type) => rev_curry (tcurry (fun x1 => .. (tcurry (fun xn (_ : tuple_type tnil) => nil)) ..)))
-      (fun (ts: list Type) => rev_curry (tcurry (fun x1 => .. (tcurry (fun xn (_ : tuple_type tnil) => nil)) ..))) _ _))
+     (SEPx (cons (atomic_shift(B := unit) (fun (_ : unit) => S2) (⊤ ∖ E) ∅ (fun x _ => fold_right_sepcon (cons SQx%I .. (cons SQy%I nil) ..)) (fun _ => Q)) (cons S1x%I .. (cons S1y%I nil) ..)))))))) ..)))
+   (rev_curry (tcurry (λne x1, .. (tcurry (λne xn, tcurry (λne (Q : mpred) (_ : tuple_type tnil),  PROP () LOCAL () (SEPx (Q :: nil))))) ..)))
+   )
   (at level 200, x1 closed binder, xn closed binder, E at level 0, S2 at level 0).
 
-Notation "'ATOMIC' 'TYPE' W 'OBJ' x 'INVS' E 'WITH' x1 , .. , xn 'PRE'  [ ] 'PROP' ( Px ; .. ; Py ) 'PARAMS' ( Lx ; .. ; Ly ) 'GLOBALS' ( Gx ; .. ; Gy ) 'SEP' ( S1x ; .. ; S1y ) '|' S2 'POST' [ tz ] 'EX' r : T , 'PROP' () 'LOCAL' ( LQx ; .. ; LQy ) 'SEP' ( SPx ; .. ; SPy ) '|' ( SQx ; .. ; SQy )" :=
-  (mk_funspec (pair nil tz) cc_default (atomic_spec_type W T)
-   (fun (ts: list Type) => rev_curry (tcurry (fun x1 => .. (tcurry (fun xn => tcurry (fun (Q : T -> mpred) (_ : tuple_type tnil) =>
+Notation "'ATOMIC' 'TYPE' W 'OBJ' x 'INVS' E 'WITH' x1 , .. , xn 'PRE'  [ ] 'PROP' ( Px ; .. ; Py ) 'PARAMS' ( Lx ; .. ; Ly ) 'GLOBALS' ( Gx ; .. ; Gy ) 'SEP' ( S1x ; .. ; S1y ) '|' S2 'POST' [ tz ] '∃' r : T , 'PROP' () 'LOCAL' ( LQx ; .. ; LQy ) 'SEP' ( SPx ; .. ; SPy ) '|' ( SQx ; .. ; SQy )" :=
+  (mk_funspec (pair nil tz) cc_default ⊤ (atomic_spec_type W T)
+   (rev_curry (tcurry (λne x1, .. (tcurry (λne xn, tcurry (λne (Q : T -> mpred) (_ : tuple_type tnil),
      PROPx (cons Px%type .. (cons Py%type nil) ..)
      (PARAMSx (cons Lx%type .. (cons Ly%type nil) ..) (GLOBALSx (cons Gx .. (cons Gy nil) ..)
-     (SEPx (cons (atomic_shift (fun x => S2) (⊤ ∖ E) ∅ (fun x r => fold_right_sepcon (cons SQx%logic .. (cons SQy%logic nil) ..)) Q) (cons S1x%logic .. (cons S1y%logic nil) ..)))))))) ..)))
-   (fun (ts: list Type) => rev_curry (tcurry (fun x1 => .. (tcurry (fun xn => tcurry (fun (Q : T -> mpred) (_ : tuple_type tnil) =>
-    @exp (environ -> mpred) _ T (fun r =>
+     (SEPx (cons (atomic_shift (fun x => S2) (⊤ ∖ E) ∅ (fun x r => fold_right_sepcon (cons SQx%I .. (cons SQy%I nil) ..)) Q) (cons S1x%I .. (cons S1y%I nil) ..)))))))) ..)))
+   (rev_curry (tcurry (λne x1, .. (tcurry (λne xn, tcurry (λne (Q : T -> mpred) (_ : tuple_type tnil),
+    bi_exist(A := T) (fun r =>
      PROP () (LOCALx (cons LQx .. (cons LQy nil) ..) ((SEPx (Q r :: cons SPx .. (cons SPy nil) ..)))))))) ..)))
-   (@atomic_spec_nonexpansive_pre' _ T _ W
-      (fun (ts: list Type) => rev_curry (tcurry (fun x1 => .. (tcurry (fun xn (_ : tuple_type tnil) => (cons Px%type .. (cons Py%type nil) ..))) ..)))
-      (fun (ts: list Type) => rev_curry (tcurry (fun x1 => .. (tcurry (fun xn (_ : tuple_type tnil) => (cons Lx%type .. (cons Ly%type nil) ..))) ..)))
-      (fun (ts: list Type) => rev_curry (tcurry (fun x1 => .. (tcurry (fun xn (_ : tuple_type tnil) => (cons Gx .. (cons Gy nil) ..))) ..)))
-      (fun (ts: list Type) => rev_curry (tcurry (fun x1 => .. (tcurry (fun xn (_ : tuple_type tnil) => (cons S1x%logic .. (cons S1y%logic nil) ..))) ..)))
-      (fun (ts: list Type) => rev_curry (tcurry (fun x1 => .. (tcurry (fun xn (_ : tuple_type tnil) x => S2)) ..)))       (fun (ts: list Type) => rev_curry (tcurry (fun x1 => .. (tcurry (fun xn (_ : tuple_type tnil) => E)) ..)))
-      (fun (ts: list Type) => rev_curry (tcurry (fun x1 => .. (tcurry (fun xn (_ : tuple_type tnil) x r => fold_right_sepcon (cons SQx%logic .. (cons SQy%logic nil) ..))) ..)))
-     _ _ _ _ _ _ _)
-  (atomic_spec_nonexpansive_post' W
-      (fun (ts: list Type) => rev_curry (tcurry (fun x1 => .. (tcurry (fun xn (_ : tuple_type tnil) r => (cons LQx%assert3 .. (cons LQy%assert3 nil) ..))) ..)))
-      (fun (ts: list Type) => rev_curry (tcurry (fun x1 => .. (tcurry (fun xn (_ : tuple_type tnil) r => (cons SPx%assert3 .. (cons SPy%assert3 nil) ..))) ..))) _ _))
+   )
   (at level 200, x1 closed binder, xn closed binder, x at level 0, E at level 0, S2 at level 0, r at level 0, T at level 0).
 
-Notation "'ATOMIC' 'TYPE' W 'OBJ' x 'INVS' E 'WITH' x1 , .. , xn 'PRE'  [ ] 'PROP' ( Px ; .. ; Py ) 'PARAMS' ( Lx ; .. ; Ly ) 'GLOBALS' ( Gx ; .. ; Gy ) 'SEP' ( S1x ; .. ; S1y ) '|' S2 'POST' [ tz ] 'EX' r : T , 'PROP' () 'LOCAL' () 'SEP' ( SPx ; .. ; SPy ) '|' ( SQx ; .. ; SQy )" :=
-  (mk_funspec (pair nil tz) cc_default (atomic_spec_type W T)
-   (fun (ts: list Type) => rev_curry (tcurry (fun x1 => .. (tcurry (fun xn => tcurry (fun (Q : T -> mpred) (_ : tuple_type tnil) =>
+Notation "'ATOMIC' 'TYPE' W 'OBJ' x 'INVS' E 'WITH' x1 , .. , xn 'PRE'  [ ] 'PROP' ( Px ; .. ; Py ) 'PARAMS' ( Lx ; .. ; Ly ) 'GLOBALS' ( Gx ; .. ; Gy ) 'SEP' ( S1x ; .. ; S1y ) '|' S2 'POST' [ tz ] '∃' r : T , 'PROP' () 'LOCAL' () 'SEP' ( SPx ; .. ; SPy ) '|' ( SQx ; .. ; SQy )" :=
+  (mk_funspec (pair nil tz) cc_default ⊤ (atomic_spec_type W T)
+   (rev_curry (tcurry (λne x1, .. (tcurry (λne xn, tcurry (λne (Q : T -> mpred) (_ : tuple_type tnil),
      PROPx (cons Px%type .. (cons Py%type nil) ..)
      (PARAMSx (cons Lx%type .. (cons Ly%type nil) ..) (GLOBALSx (cons Gx .. (cons Gy nil) ..)
-     (SEPx (cons (atomic_shift (fun x => S2) (⊤ ∖ E) ∅ (fun x r => fold_right_sepcon (cons SQx%logic .. (cons SQy%logic nil) ..)) Q) (cons S1x%logic .. (cons S1y%logic nil) ..)))))))) ..)))
-   (fun (ts: list Type) => rev_curry (tcurry (fun x1 => .. (tcurry (fun xn => tcurry (fun (Q : T -> mpred) (_ : tuple_type tnil) =>
-    @exp (environ -> mpred) _ T (fun r =>
+     (SEPx (cons (atomic_shift (fun x => S2) (⊤ ∖ E) ∅ (fun x r => fold_right_sepcon (cons SQx%I .. (cons SQy%I nil) ..)) Q) (cons S1x%I .. (cons S1y%I nil) ..)))))))) ..)))
+   (rev_curry (tcurry (λne x1, .. (tcurry (λne xn, tcurry (λne (Q : T -> mpred) (_ : tuple_type tnil),
+    bi_exist(A := T) (fun r =>
      PROP () (LOCAL () (SEPx (Q r :: cons SPx .. (cons SPy nil) ..))))))) ..)))
-   (@atomic_spec_nonexpansive_pre' _ T _ W
-      (fun (ts: list Type) => rev_curry (tcurry (fun x1 => .. (tcurry (fun xn (_ : tuple_type tnil) => (cons Px%type .. (cons Py%type nil) ..))) ..)))
-      (fun (ts: list Type) => rev_curry (tcurry (fun x1 => .. (tcurry (fun xn (_ : tuple_type tnil) => (cons Lx%type .. (cons Ly%type nil) ..))) ..)))
-      (fun (ts: list Type) => rev_curry (tcurry (fun x1 => .. (tcurry (fun xn (_ : tuple_type tnil) => (cons Gx .. (cons Gy nil) ..))) ..)))
-      (fun (ts: list Type) => rev_curry (tcurry (fun x1 => .. (tcurry (fun xn (_ : tuple_type tnil) => (cons S1x%logic .. (cons S1y%logic nil) ..))) ..)))
-      (fun (ts: list Type) => rev_curry (tcurry (fun x1 => .. (tcurry (fun xn (_ : tuple_type tnil) x => S2)) ..)))       (fun (ts: list Type) => rev_curry (tcurry (fun x1 => .. (tcurry (fun xn (_ : tuple_type tnil) => E)) ..)))
-      (fun (ts: list Type) => rev_curry (tcurry (fun x1 => .. (tcurry (fun xn (_ : tuple_type tnil) x r => fold_right_sepcon (cons SQx%logic .. (cons SQy%logic nil) ..))) ..)))
-     _ _ _ _ _ _ _)
-  (atomic_spec_nonexpansive_post' W
-      (fun (ts: list Type) => rev_curry (tcurry (fun x1 => .. (tcurry (fun xn (_ : tuple_type tnil) r => nil)) ..)))
-      (fun (ts: list Type) => rev_curry (tcurry (fun x1 => .. (tcurry (fun xn (_ : tuple_type tnil) r => (cons SPx%assert5%assert3 .. (cons SPy%assert5%assert3 nil) ..))) ..))) _ _))
+   )
   (at level 200, x1 closed binder, xn closed binder, x at level 0, E at level 0, S2 at level 0, r at level 0, T at level 0).
 
 Notation "'ATOMIC' 'TYPE' W 'OBJ' x 'INVS' E 'WITH' x1 , .. , xn 'PRE'  [ ] 'PROP' ( Px ; .. ; Py ) 'PARAMS ( Lx ; .. ; Ly ) 'GLOBALS' ( Gx ; .. ; Gy ) 'SEP' ( S1x ; .. ; S1y ) '|' S2 'POST' [ tz ] 'PROP' () 'LOCAL' ( LQx ; .. ; LQy ) 'SEP' ( SPx ; .. ; SPy ) '|' ( SQx ; .. ; SQy )" :=
-  (mk_funspec (pair nil tz) cc_default (atomic_spec_type0 W)
-   (fun (ts: list Type) => rev_curry (tcurry (fun x1 => .. (tcurry (fun xn => tcurry (fun (Q : mpred) (_ : tuple_type tnil) =>
-     PROPx (cons Px%type .. (cons Py%type nil) ..)
+  (mk_funspec (pair nil tz) cc_default ⊤ (atomic_spec_type0 W)
+   (rev_curry (tcurry (λne x1, .. (tcurry (λne xn, tcurry (λne (Q : mpred) (_ : tuple_type tnil),  PROPx (cons Px%type .. (cons Py%type nil) ..)
      (PARAMSx (cons Lx%type .. (cons Ly%type nil) ..) (GLOBALSx (cons Gx .. (cons Gy nil) ..)
-     (SEPx (cons (atomic_shift(B := unit) (fun x => S2) (⊤ ∖ E) ∅ (fun x _ => fold_right_sepcon (cons SQx%logic .. (cons SQy%logic nil) ..)) (fun _ => Q)) (cons S1x%logic .. (cons S1y%logic nil) ..)))))))) ..)))
-   (fun (ts: list Type) => rev_curry (tcurry (fun x1 => .. (tcurry (fun xn => tcurry (fun (Q : mpred) (_ : tuple_type tnil) =>
-     PROP () (LOCALx (cons LQx .. (cons LQy nil) ..) (SEPx (Q :: cons SPx .. (cons SPy nil) ..)))))) ..)))
-   (@atomic_spec_nonexpansive_pre0 _ W
-      (fun (ts: list Type) => rev_curry (tcurry (fun x1 => .. (tcurry (fun xn (_ : tuple_type tnil) => (cons Px%type .. (cons Py%type nil) ..))) ..)))
-      (fun (ts: list Type) => rev_curry (tcurry (fun x1 => .. (tcurry (fun xn (_ : tuple_type tnil) => (cons Lx%type .. (cons Ly%type nil) ..))) ..)))
-      (fun (ts: list Type) => rev_curry (tcurry (fun x1 => .. (tcurry (fun xn (_ : tuple_type tnil) => (cons Gx .. (cons Gy nil) ..))) ..)))
-      (fun (ts: list Type) => rev_curry (tcurry (fun x1 => .. (tcurry (fun xn (_ : tuple_type tnil) => (cons S1x%logic .. (cons S1y%logic nil) ..))) ..)))
-      (fun (ts: list Type) => rev_curry (tcurry (fun x1 => .. (tcurry (fun xn (_ : tuple_type tnil) x => S2)) ..)))       (fun (ts: list Type) => rev_curry (tcurry (fun x1 => .. (tcurry (fun xn (_ : tuple_type tnil) => E)) ..)))
-      (fun (ts: list Type) => rev_curry (tcurry (fun x1 => .. (tcurry (fun xn (_ : tuple_type tnil) x _ => fold_right_sepcon (cons SQx%logic .. (cons SQy%logic nil) ..))) ..)))
-     _ _ _ _ _ _ _)
-  (atomic_spec_nonexpansive_post0 W
-      (fun (ts: list Type) => rev_curry (tcurry (fun x1 => .. (tcurry (fun xn (_ : tuple_type tnil) => (cons LQx%assert3 .. (cons LQy%assert3 nil) ..))) ..)))
-      (fun (ts: list Type) => rev_curry (tcurry (fun x1 => .. (tcurry (fun xn (_ : tuple_type tnil) => (cons SPx%assert3 .. (cons SPy%assert3 nil) ..))) ..))) _ _))
+     (SEPx (cons (atomic_shift(B := unit) (fun x => S2) (⊤ ∖ E) ∅ (fun x _ => fold_right_sepcon (cons SQx%I .. (cons SQy%I nil) ..)) (fun _ => Q)) (cons S1x%I .. (cons S1y%I nil) ..)))))))) ..)))
+   (rev_curry (tcurry (λne x1, .. (tcurry (λne xn, tcurry (λne (Q : mpred) (_ : tuple_type tnil),  PROP () (LOCALx (cons LQx .. (cons LQy nil) ..) (SEPx (Q :: cons SPx .. (cons SPy nil) ..)))))) ..)))
+   )
   (at level 200, x1 closed binder, xn closed binder, x at level 0, E at level 0, S2 at level 0).
 
 Notation "'ATOMIC' 'TYPE' W 'OBJ' x 'INVS' E 'WITH' x1 , .. , xn 'PRE'  [ ] 'PROP' ( Px ; .. ; Py ) 'PARAMS' ( Lx ; .. ; Ly ) 'GLOBALS' ( Gx ; .. ; Gy ) 'SEP' ( S1x ; .. ; S1y ) '|' S2 'POST' [ tz ] 'PROP' () 'LOCAL' () 'SEP' ( SPx ; .. ; SPy ) '|' ( SQx ; .. ; SQy )" :=
-  (mk_funspec (pair nil tz) cc_default (atomic_spec_type0 W)
-   (fun (ts: list Type) => rev_curry (tcurry (fun x1 => .. (tcurry (fun xn => tcurry (fun (Q : mpred) (_ : tuple_type tnil) =>
-     PROPx (cons Px%type .. (cons Py%type nil) ..)
+  (mk_funspec (pair nil tz) cc_default ⊤ (atomic_spec_type0 W)
+   (rev_curry (tcurry (λne x1, .. (tcurry (λne xn, tcurry (λne (Q : mpred) (_ : tuple_type tnil),  PROPx (cons Px%type .. (cons Py%type nil) ..)
      (PARAMSx (cons Lx%type .. (cons Ly%type nil) ..) (GLOBALSx (cons Gx .. (cons Gy nil) ..)
-     (SEPx (cons (atomic_shift(B := unit) (fun x => S2) (⊤ ∖ E) ∅ (fun x _ => fold_right_sepcon (cons SQx%logic .. (cons SQy%logic nil) ..)) (fun _ => Q)) (cons S1x%logic .. (cons S1y%logic nil) ..)))))))) ..)))
-   (fun (ts: list Type) => rev_curry (tcurry (fun x1 => .. (tcurry (fun xn => tcurry (fun (Q : mpred) (_ : tuple_type tnil) =>
-     PROP () LOCAL () (SEPx (Q :: cons SPx .. (cons SPy nil) ..))))) ..)))
-   (@atomic_spec_nonexpansive_pre0 _ W
-      (fun (ts: list Type) => rev_curry (tcurry (fun x1 => .. (tcurry (fun xn (_ : tuple_type tnil) => (cons Px%type .. (cons Py%type nil) ..))) ..)))
-      (fun (ts: list Type) => rev_curry (tcurry (fun x1 => .. (tcurry (fun xn (_ : tuple_type tnil) => (cons Lx%type .. (cons Ly%type nil) ..))) ..)))
-      (fun (ts: list Type) => rev_curry (tcurry (fun x1 => .. (tcurry (fun xn (_ : tuple_type tnil) => (cons Gx .. (cons Gy nil) ..))) ..)))
-      (fun (ts: list Type) => rev_curry (tcurry (fun x1 => .. (tcurry (fun xn (_ : tuple_type tnil) => (cons S1x%logic .. (cons S1y%logic nil) ..))) ..)))
-      (fun (ts: list Type) => rev_curry (tcurry (fun x1 => .. (tcurry (fun xn (_ : tuple_type tnil) x => S2)) ..)))       (fun (ts: list Type) => rev_curry (tcurry (fun x1 => .. (tcurry (fun xn (_ : tuple_type tnil) => E)) ..)))
-      (fun (ts: list Type) => rev_curry (tcurry (fun x1 => .. (tcurry (fun xn (_ : tuple_type tnil) x _ => fold_right_sepcon (cons SQx%logic .. (cons SQy%logic nil) ..))) ..)))
-     _ _ _ _ _ _ _)
-  (atomic_spec_nonexpansive_post0 W
-      (fun (ts: list Type) => rev_curry (tcurry (fun x1 => .. (tcurry (fun xn (_ : tuple_type tnil) => nil)) ..)))
-      (fun (ts: list Type) => rev_curry (tcurry (fun x1 => .. (tcurry (fun xn (_ : tuple_type tnil) => (cons SPx%assert5%assert3 .. (cons SPy%assert5%assert3 nil) ..))) ..))) _ _))
+     (SEPx (cons (atomic_shift(B := unit) (fun x => S2) (⊤ ∖ E) ∅ (fun x _ => fold_right_sepcon (cons SQx%I .. (cons SQy%I nil) ..)) (fun _ => Q)) (cons S1x%I .. (cons S1y%I nil) ..)))))))) ..)))
+   (rev_curry (tcurry (λne x1, .. (tcurry (λne xn, tcurry (λne (Q : mpred) (_ : tuple_type tnil),  PROP () LOCAL () (SEPx (Q :: cons SPx .. (cons SPy nil) ..))))) ..)))
+   )
   (at level 200, x1 closed binder, xn closed binder, x at level 0, E at level 0, S2 at level 0).
 
-Notation "'ATOMIC' 'TYPE' W 'OBJ' x 'INVS' E 'WITH' x1 , .. , xn 'PRE'  [ u , .. , v ] 'PROP' ( Px ; .. ; Py ) 'PARAMS' () 'GLOBALS' ( Gx ; .. ; Gy ) 'SEP' ( S1x ; .. ; S1y ) '|' S2 'POST' [ tz ] 'EX' r : T , 'PROP' () 'LOCAL' ( LQx ; .. ; LQy ) 'SEP' ( SPx ; .. ; SPy ) '|' ( SQx ; .. ; SQy )" :=
-  (mk_funspec (pair (cons u%type .. (cons v%type nil) ..) tz) cc_default (atomic_spec_type W T)
-   (fun (ts: list Type) => rev_curry (tcurry (fun x1 => .. (tcurry (fun xn => tcurry (fun (Q : T -> mpred) (_ : tuple_type tnil) =>
+Notation "'ATOMIC' 'TYPE' W 'OBJ' x 'INVS' E 'WITH' x1 , .. , xn 'PRE'  [ u , .. , v ] 'PROP' ( Px ; .. ; Py ) 'PARAMS' () 'GLOBALS' ( Gx ; .. ; Gy ) 'SEP' ( S1x ; .. ; S1y ) '|' S2 'POST' [ tz ] '∃' r : T , 'PROP' () 'LOCAL' ( LQx ; .. ; LQy ) 'SEP' ( SPx ; .. ; SPy ) '|' ( SQx ; .. ; SQy )" :=
+  (mk_funspec (pair (cons u%type .. (cons v%type nil) ..) tz) cc_default ⊤ (atomic_spec_type W T)
+   (rev_curry (tcurry (λne x1, .. (tcurry (λne xn, tcurry (λne (Q : T -> mpred) (_ : tuple_type tnil),
      PROPx (cons Px%type .. (cons Py%type nil) ..)
      (PARAMSx nil (GLOBALSx (cons Gx .. (cons Gy nil) ..)
-     (SEPx (cons (atomic_shift (fun x => S2) (⊤ ∖ E) ∅ (fun x r => fold_right_sepcon (cons SQx%logic .. (cons SQy%logic nil) ..)) Q) (cons S1x%logic .. (cons S1y%logic nil) ..)))))))) ..)))
-   (fun (ts: list Type) => rev_curry (tcurry (fun x1 => .. (tcurry (fun xn => tcurry (fun (Q : T -> mpred) (_ : tuple_type tnil) =>
-    @exp (environ -> mpred) _ T (fun r =>
+     (SEPx (cons (atomic_shift (fun x => S2) (⊤ ∖ E) ∅ (fun x r => fold_right_sepcon (cons SQx%I .. (cons SQy%I nil) ..)) Q) (cons S1x%I .. (cons S1y%I nil) ..)))))))) ..)))
+   (rev_curry (tcurry (λne x1, .. (tcurry (λne xn, tcurry (λne (Q : T -> mpred) (_ : tuple_type tnil),
+    bi_exist(A := T) (fun r =>
      PROP () (LOCALx (cons LQx .. (cons LQy nil) ..) ((SEPx (Q r :: cons SPx .. (cons SPy nil) ..)))))))) ..)))
-   (@atomic_spec_nonexpansive_pre' _ T _ W
-      (fun (ts: list Type) => rev_curry (tcurry (fun x1 => .. (tcurry (fun xn (_ : tuple_type tnil) => (cons Px%type .. (cons Py%type nil) ..))) ..)))
-      (fun (ts: list Type) => rev_curry (tcurry (fun x1 => .. (tcurry (fun xn (_ : tuple_type tnil) => nil)) ..)))
-      (fun (ts: list Type) => rev_curry (tcurry (fun x1 => .. (tcurry (fun xn (_ : tuple_type tnil) => (cons Gx .. (cons Gy nil) ..))) ..)))
-      (fun (ts: list Type) => rev_curry (tcurry (fun x1 => .. (tcurry (fun xn (_ : tuple_type tnil) => (cons S1x%logic .. (cons S1y%logic nil) ..))) ..)))
-      (fun (ts: list Type) => rev_curry (tcurry (fun x1 => .. (tcurry (fun xn (_ : tuple_type tnil) x => S2)) ..)))       (fun (ts: list Type) => rev_curry (tcurry (fun x1 => .. (tcurry (fun xn (_ : tuple_type tnil) => E)) ..)))
-      (fun (ts: list Type) => rev_curry (tcurry (fun x1 => .. (tcurry (fun xn (_ : tuple_type tnil) x r => fold_right_sepcon (cons SQx%logic .. (cons SQy%logic nil) ..))) ..)))
-     _ _ _ _ _ _ _)
-  (atomic_spec_nonexpansive_post' W
-      (fun (ts: list Type) => rev_curry (tcurry (fun x1 => .. (tcurry (fun xn (_ : tuple_type tnil) r => (cons LQx%assert3 .. (cons LQy%assert3 nil) ..))) ..)))
-      (fun (ts: list Type) => rev_curry (tcurry (fun x1 => .. (tcurry (fun xn (_ : tuple_type tnil) r => (cons SPx%assert3 .. (cons SPy%assert3 nil) ..))) ..))) _ _))
+   )
   (at level 200, x1 closed binder, xn closed binder, x at level 0, E at level 0, S2 at level 0, r at level 0, T at level 0).
 
-Notation "'ATOMIC' 'TYPE' W 'OBJ' x 'INVS' E 'WITH' x1 , .. , xn 'PRE'  [ u , .. , v ] 'PROP' ( Px ; .. ; Py ) 'PARAMS' () 'GLOBALS' ( Gx ; .. ; Gy ) 'SEP' ( S1x ; .. ; S1y ) '|' S2 'POST' [ tz ] 'EX' r : T , 'PROP' () 'LOCAL' () 'SEP' ( SPx ; .. ; SPy ) '|' ( SQx ; .. ; SQy )" :=
-  (mk_funspec (pair (cons u%type .. (cons v%type nil) ..) tz) cc_default (atomic_spec_type W T)
-   (fun (ts: list Type) => rev_curry (tcurry (fun x1 => .. (tcurry (fun xn => tcurry (fun (Q : T -> mpred) (_ : tuple_type tnil) =>
+Notation "'ATOMIC' 'TYPE' W 'OBJ' x 'INVS' E 'WITH' x1 , .. , xn 'PRE'  [ u , .. , v ] 'PROP' ( Px ; .. ; Py ) 'PARAMS' () 'GLOBALS' ( Gx ; .. ; Gy ) 'SEP' ( S1x ; .. ; S1y ) '|' S2 'POST' [ tz ] '∃' r : T , 'PROP' () 'LOCAL' () 'SEP' ( SPx ; .. ; SPy ) '|' ( SQx ; .. ; SQy )" :=
+  (mk_funspec (pair (cons u%type .. (cons v%type nil) ..) tz) cc_default ⊤ (atomic_spec_type W T)
+   (rev_curry (tcurry (λne x1, .. (tcurry (λne xn, tcurry (λne (Q : T -> mpred) (_ : tuple_type tnil),
      PROPx (cons Px%type .. (cons Py%type nil) ..)
      (PARAMSx nil (GLOBALSx (cons Gx .. (cons Gy nil) ..)
-     (SEPx (cons (atomic_shift (fun x => S2) (⊤ ∖ E) ∅ (fun x r => fold_right_sepcon (cons SQx%logic .. (cons SQy%logic nil) ..)) Q) (cons S1x%logic .. (cons S1y%logic nil) ..)))))))) ..)))
-   (fun (ts: list Type) => rev_curry (tcurry (fun x1 => .. (tcurry (fun xn => tcurry (fun (Q : T -> mpred) (_ : tuple_type tnil) =>
-    @exp (environ -> mpred) _ T (fun r =>
+     (SEPx (cons (atomic_shift (fun x => S2) (⊤ ∖ E) ∅ (fun x r => fold_right_sepcon (cons SQx%I .. (cons SQy%I nil) ..)) Q) (cons S1x%I .. (cons S1y%I nil) ..)))))))) ..)))
+   (rev_curry (tcurry (λne x1, .. (tcurry (λne xn, tcurry (λne (Q : T -> mpred) (_ : tuple_type tnil),
+    bi_exist(A := T) (fun r =>
      PROP () (LOCAL () (SEPx (Q r :: cons SPx .. (cons SPy nil) ..))))))) ..)))
-   (@atomic_spec_nonexpansive_pre' _ T _ W
-      (fun (ts: list Type) => rev_curry (tcurry (fun x1 => .. (tcurry (fun xn (_ : tuple_type tnil) => (cons Px%type .. (cons Py%type nil) ..))) ..)))
-      (fun (ts: list Type) => rev_curry (tcurry (fun x1 => .. (tcurry (fun xn (_ : tuple_type tnil) => nil)) ..)))
-      (fun (ts: list Type) => rev_curry (tcurry (fun x1 => .. (tcurry (fun xn (_ : tuple_type tnil) => (cons Gx .. (cons Gy nil) ..))) ..)))
-      (fun (ts: list Type) => rev_curry (tcurry (fun x1 => .. (tcurry (fun xn (_ : tuple_type tnil) => (cons S1x%logic .. (cons S1y%logic nil) ..))) ..)))
-      (fun (ts: list Type) => rev_curry (tcurry (fun x1 => .. (tcurry (fun xn (_ : tuple_type tnil) x => S2)) ..)))       (fun (ts: list Type) => rev_curry (tcurry (fun x1 => .. (tcurry (fun xn (_ : tuple_type tnil) => E)) ..)))
-      (fun (ts: list Type) => rev_curry (tcurry (fun x1 => .. (tcurry (fun xn (_ : tuple_type tnil) x r => fold_right_sepcon (cons SQx%logic .. (cons SQy%logic nil) ..))) ..)))
-     _ _ _ _ _ _ _)
-  (atomic_spec_nonexpansive_post' W
-      (fun (ts: list Type) => rev_curry (tcurry (fun x1 => .. (tcurry (fun xn (_ : tuple_type tnil) r => nil)) ..)))
-      (fun (ts: list Type) => rev_curry (tcurry (fun x1 => .. (tcurry (fun xn (_ : tuple_type tnil) r => (cons SPx%assert5%assert3 .. (cons SPy%assert5%assert3 nil) ..))) ..))) _ _))
+   )
   (at level 200, x1 closed binder, xn closed binder, x at level 0, E at level 0, S2 at level 0, r at level 0, T at level 0).
 
 Notation "'ATOMIC' 'TYPE' W 'OBJ' x 'INVS' E 'WITH' x1 , .. , xn 'PRE'  [ u , .. , v ] 'PROP' ( Px ; .. ; Py ) 'PARAMS' () 'GLOBALS' ( Gx ; .. ; Gy ) 'SEP' ( S1x ; .. ; S1y ) '|' S2 'POST' [ tz ] 'PROP' () 'LOCAL' ( LQx ; .. ; LQy ) 'SEP' ( SPx ; .. ; SPy ) '|' ( SQx ; .. ; SQy )" :=
-  (mk_funspec (pair (cons u%type .. (cons v%type nil) ..) tz) cc_default (atomic_spec_type0 W)
-   (fun (ts: list Type) => rev_curry (tcurry (fun x1 => .. (tcurry (fun xn => tcurry (fun (Q : mpred) (_ : tuple_type tnil) =>
-     PROPx (cons Px%type .. (cons Py%type nil) ..)
+  (mk_funspec (pair (cons u%type .. (cons v%type nil) ..) tz) cc_default ⊤ (atomic_spec_type0 W)
+   (rev_curry (tcurry (λne x1, .. (tcurry (λne xn, tcurry (λne (Q : mpred) (_ : tuple_type tnil),  PROPx (cons Px%type .. (cons Py%type nil) ..)
      (PARAMSx nil (GLOBALSx (cons Gx .. (cons Gy nil) ..)
-     (SEPx (cons (atomic_shift(B := unit) (fun x => S2) (⊤ ∖ E) ∅ (fun x _ => fold_right_sepcon (cons SQx%logic .. (cons SQy%logic nil) ..)) (fun _ => Q)) (cons S1x%logic .. (cons S1y%logic nil) ..)))))))) ..)))
-   (fun (ts: list Type) => rev_curry (tcurry (fun x1 => .. (tcurry (fun xn => tcurry (fun (Q : mpred) (_ : tuple_type tnil) =>
-     PROP () (LOCALx (cons LQx .. (cons LQy nil) ..) (SEPx (Q :: cons SPx .. (cons SPy nil) ..)))))) ..)))
-   (@atomic_spec_nonexpansive_pre0 _ W
-      (fun (ts: list Type) => rev_curry (tcurry (fun x1 => .. (tcurry (fun xn (_ : tuple_type tnil) => (cons Px%type .. (cons Py%type nil) ..))) ..)))
-      (fun (ts: list Type) => rev_curry (tcurry (fun x1 => .. (tcurry (fun xn (_ : tuple_type tnil) => nil)) ..)))
-      (fun (ts: list Type) => rev_curry (tcurry (fun x1 => .. (tcurry (fun xn (_ : tuple_type tnil) => (cons Gx .. (cons Gy nil) ..))) ..)))
-      (fun (ts: list Type) => rev_curry (tcurry (fun x1 => .. (tcurry (fun xn (_ : tuple_type tnil) => (cons S1x%logic .. (cons S1y%logic nil) ..))) ..)))
-      (fun (ts: list Type) => rev_curry (tcurry (fun x1 => .. (tcurry (fun xn (_ : tuple_type tnil) x => S2)) ..)))       (fun (ts: list Type) => rev_curry (tcurry (fun x1 => .. (tcurry (fun xn (_ : tuple_type tnil) => E)) ..)))
-      (fun (ts: list Type) => rev_curry (tcurry (fun x1 => .. (tcurry (fun xn (_ : tuple_type tnil) x _ => fold_right_sepcon (cons SQx%logic .. (cons SQy%logic nil) ..))) ..)))
-     _ _ _ _ _ _ _)
-  (atomic_spec_nonexpansive_post0 W
-      (fun (ts: list Type) => rev_curry (tcurry (fun x1 => .. (tcurry (fun xn (_ : tuple_type tnil) => (cons LQx%assert3 .. (cons LQy%assert3 nil) ..))) ..)))
-      (fun (ts: list Type) => rev_curry (tcurry (fun x1 => .. (tcurry (fun xn (_ : tuple_type tnil) => (cons SPx%assert3 .. (cons SPy%assert3 nil) ..))) ..))) _ _))
+     (SEPx (cons (atomic_shift(B := unit) (fun x => S2) (⊤ ∖ E) ∅ (fun x _ => fold_right_sepcon (cons SQx%I .. (cons SQy%I nil) ..)) (fun _ => Q)) (cons S1x%I .. (cons S1y%I nil) ..)))))))) ..)))
+   (rev_curry (tcurry (λne x1, .. (tcurry (λne xn, tcurry (λne (Q : mpred) (_ : tuple_type tnil),  PROP () (LOCALx (cons LQx .. (cons LQy nil) ..) (SEPx (Q :: cons SPx .. (cons SPy nil) ..)))))) ..)))
+   )
   (at level 200, x1 closed binder, xn closed binder, x at level 0, E at level 0, S2 at level 0).
 
 Notation "'ATOMIC' 'TYPE' W 'OBJ' x 'INVS' E 'WITH' x1 , .. , xn 'PRE'  [ u , .. , v ] 'PROP' ( Px ; .. ; Py ) 'PARAMS' () 'GLOBALS' ( Gx ; .. ; Gy ) 'SEP' ( S1x ; .. ; S1y ) '|' S2 'POST' [ tz ] 'PROP' () 'LOCAL' () 'SEP' ( SPx ; .. ; SPy ) '|' ( SQx ; .. ; SQy )" :=
-  (mk_funspec (pair (cons u%type .. (cons v%type nil) ..) tz) cc_default (atomic_spec_type0 W)
-   (fun (ts: list Type) => rev_curry (tcurry (fun x1 => .. (tcurry (fun xn => tcurry (fun (Q : mpred) (_ : tuple_type tnil) =>
-     PROPx (cons Px%type .. (cons Py%type nil) ..)
+  (mk_funspec (pair (cons u%type .. (cons v%type nil) ..) tz) cc_default ⊤ (atomic_spec_type0 W)
+   (rev_curry (tcurry (λne x1, .. (tcurry (λne xn, tcurry (λne (Q : mpred) (_ : tuple_type tnil),  PROPx (cons Px%type .. (cons Py%type nil) ..)
      (PARAMSx nil (GLOBALSx (cons Gx .. (cons Gy nil) ..)
-     (SEPx (cons (atomic_shift(B := unit) (fun x => S2) (⊤ ∖ E) ∅ (fun x _ => fold_right_sepcon (cons SQx%logic .. (cons SQy%logic nil) ..)) (fun _ => Q)) (cons S1x%logic .. (cons S1y%logic nil) ..)))))))) ..)))
-   (fun (ts: list Type) => rev_curry (tcurry (fun x1 => .. (tcurry (fun xn => tcurry (fun (Q : mpred) (_ : tuple_type tnil) =>
-     PROP () LOCAL () (SEPx (Q :: cons SPx .. (cons SPy nil) ..))))) ..)))
-   (@atomic_spec_nonexpansive_pre0 _ W
-      (fun (ts: list Type) => rev_curry (tcurry (fun x1 => .. (tcurry (fun xn (_ : tuple_type tnil) => (cons Px%type .. (cons Py%type nil) ..))) ..)))
-      (fun (ts: list Type) => rev_curry (tcurry (fun x1 => .. (tcurry (fun xn (_ : tuple_type tnil) => nil)) ..)))
-      (fun (ts: list Type) => rev_curry (tcurry (fun x1 => .. (tcurry (fun xn (_ : tuple_type tnil) => (cons Gx .. (cons Gy nil) ..))) ..)))
-      (fun (ts: list Type) => rev_curry (tcurry (fun x1 => .. (tcurry (fun xn (_ : tuple_type tnil) => (cons S1x%logic .. (cons S1y%logic nil) ..))) ..)))
-      (fun (ts: list Type) => rev_curry (tcurry (fun x1 => .. (tcurry (fun xn (_ : tuple_type tnil) x => S2)) ..)))       (fun (ts: list Type) => rev_curry (tcurry (fun x1 => .. (tcurry (fun xn (_ : tuple_type tnil) => E)) ..)))
-      (fun (ts: list Type) => rev_curry (tcurry (fun x1 => .. (tcurry (fun xn (_ : tuple_type tnil) x _ => fold_right_sepcon (cons SQx%logic .. (cons SQy%logic nil) ..))) ..)))
-     _ _ _ _ _ _ _)
-  (atomic_spec_nonexpansive_post0 W
-      (fun (ts: list Type) => rev_curry (tcurry (fun x1 => .. (tcurry (fun xn (_ : tuple_type tnil) => nil)) ..)))
-      (fun (ts: list Type) => rev_curry (tcurry (fun x1 => .. (tcurry (fun xn (_ : tuple_type tnil) => (cons SPx%assert5%assert3 .. (cons SPy%assert5%assert3 nil) ..))) ..))) _ _))
+     (SEPx (cons (atomic_shift(B := unit) (fun x => S2) (⊤ ∖ E) ∅ (fun x _ => fold_right_sepcon (cons SQx%I .. (cons SQy%I nil) ..)) (fun _ => Q)) (cons S1x%I .. (cons S1y%I nil) ..)))))))) ..)))
+   (rev_curry (tcurry (λne x1, .. (tcurry (λne xn, tcurry (λne (Q : mpred) (_ : tuple_type tnil),  PROP () LOCAL () (SEPx (Q :: cons SPx .. (cons SPy nil) ..))))) ..)))
+   )
   (at level 200, x1 closed binder, xn closed binder, x at level 0, E at level 0, S2 at level 0).
 
-Notation "'ATOMIC' 'TYPE' W 'OBJ' x 'INVS' E 'WITH' x1 , .. , xn 'PRE'  [ ] 'PROP' ( Px ; .. ; Py ) 'PARAMS' () 'GLOBALS' ( Gx ; .. ; Gy ) 'SEP' ( S1x ; .. ; S1y ) '|' S2 'POST' [ tz ] 'EX' r : T , 'PROP' () 'LOCAL' ( LQx ; .. ; LQy ) 'SEP' ( SPx ; .. ; SPy ) '|' ( SQx ; .. ; SQy )" :=
-  (mk_funspec (pair nil tz) cc_default (atomic_spec_type W T)
-   (fun (ts: list Type) => rev_curry (tcurry (fun x1 => .. (tcurry (fun xn => tcurry (fun (Q : T -> mpred) (_ : tuple_type tnil) =>
+Notation "'ATOMIC' 'TYPE' W 'OBJ' x 'INVS' E 'WITH' x1 , .. , xn 'PRE'  [ ] 'PROP' ( Px ; .. ; Py ) 'PARAMS' () 'GLOBALS' ( Gx ; .. ; Gy ) 'SEP' ( S1x ; .. ; S1y ) '|' S2 'POST' [ tz ] '∃' r : T , 'PROP' () 'LOCAL' ( LQx ; .. ; LQy ) 'SEP' ( SPx ; .. ; SPy ) '|' ( SQx ; .. ; SQy )" :=
+  (mk_funspec (pair nil tz) cc_default ⊤ (atomic_spec_type W T)
+   (rev_curry (tcurry (λne x1, .. (tcurry (λne xn, tcurry (λne (Q : T -> mpred) (_ : tuple_type tnil),
      PROPx (cons Px%type .. (cons Py%type nil) ..)
      (PARAMSx nil (GLOBALSx (cons Gx .. (cons Gy nil) ..)
-     (SEPx (cons (atomic_shift (fun x => S2) (⊤ ∖ E) ∅ (fun x r => fold_right_sepcon (cons SQx%logic .. (cons SQy%logic nil) ..)) Q) (cons S1x%logic .. (cons S1y%logic nil) ..)))))))) ..)))
-   (fun (ts: list Type) => rev_curry (tcurry (fun x1 => .. (tcurry (fun xn => tcurry (fun (Q : T -> mpred) (_ : tuple_type tnil) =>
-    @exp (environ -> mpred) _ T (fun r =>
+     (SEPx (cons (atomic_shift (fun x => S2) (⊤ ∖ E) ∅ (fun x r => fold_right_sepcon (cons SQx%I .. (cons SQy%I nil) ..)) Q) (cons S1x%I .. (cons S1y%I nil) ..)))))))) ..)))
+   (rev_curry (tcurry (λne x1, .. (tcurry (λne xn, tcurry (λne (Q : T -> mpred) (_ : tuple_type tnil),
+    bi_exist(A := T) (fun r =>
      PROP () (LOCALx (cons LQx .. (cons LQy nil) ..) ((SEPx (Q r :: cons SPx .. (cons SPy nil) ..)))))))) ..)))
-   (@atomic_spec_nonexpansive_pre' _ T _ W
-      (fun (ts: list Type) => rev_curry (tcurry (fun x1 => .. (tcurry (fun xn (_ : tuple_type tnil) => (cons Px%type .. (cons Py%type nil) ..))) ..)))
-      (fun (ts: list Type) => rev_curry (tcurry (fun x1 => .. (tcurry (fun xn (_ : tuple_type tnil) => nil)) ..)))
-      (fun (ts: list Type) => rev_curry (tcurry (fun x1 => .. (tcurry (fun xn (_ : tuple_type tnil) => (cons Gx .. (cons Gy nil) ..))) ..)))
-      (fun (ts: list Type) => rev_curry (tcurry (fun x1 => .. (tcurry (fun xn (_ : tuple_type tnil) => (cons S1x%logic .. (cons S1y%logic nil) ..))) ..)))
-      (fun (ts: list Type) => rev_curry (tcurry (fun x1 => .. (tcurry (fun xn (_ : tuple_type tnil) x => S2)) ..)))       (fun (ts: list Type) => rev_curry (tcurry (fun x1 => .. (tcurry (fun xn (_ : tuple_type tnil) => E)) ..)))
-      (fun (ts: list Type) => rev_curry (tcurry (fun x1 => .. (tcurry (fun xn (_ : tuple_type tnil) x r => fold_right_sepcon (cons SQx%logic .. (cons SQy%logic nil) ..))) ..)))
-     _ _ _ _ _ _ _)
-  (atomic_spec_nonexpansive_post' W
-      (fun (ts: list Type) => rev_curry (tcurry (fun x1 => .. (tcurry (fun xn (_ : tuple_type tnil) r => (cons LQx%assert3 .. (cons LQy%assert3 nil) ..))) ..)))
-      (fun (ts: list Type) => rev_curry (tcurry (fun x1 => .. (tcurry (fun xn (_ : tuple_type tnil) r => (cons SPx%assert3 .. (cons SPy%assert3 nil) ..))) ..))) _ _))
+   )
   (at level 200, x1 closed binder, xn closed binder, x at level 0, E at level 0, S2 at level 0, r at level 0, T at level 0).
 
-Notation "'ATOMIC' 'TYPE' W 'OBJ' x 'INVS' E 'WITH' x1 , .. , xn 'PRE'  [ ] 'PROP' () 'PARAMS' () 'GLOBALS' ( Gx ; .. ; Gy ) 'SEP' () '|' S2 'POST' [ tz ] 'EX' r : T , 'PROP' () 'LOCAL' ( LQx ; .. ; LQy ) 'SEP' () '|' ( SQx ; .. ; SQy )" :=
-  (mk_funspec (pair nil tz) cc_default (atomic_spec_type W T)
-   (fun (ts: list Type) => rev_curry (tcurry (fun x1 => .. (tcurry (fun xn => tcurry (fun (Q : T -> mpred) (_ : tuple_type tnil) =>
+Notation "'ATOMIC' 'TYPE' W 'OBJ' x 'INVS' E 'WITH' x1 , .. , xn 'PRE'  [ ] 'PROP' () 'PARAMS' () 'GLOBALS' ( Gx ; .. ; Gy ) 'SEP' () '|' S2 'POST' [ tz ] '∃' r : T , 'PROP' () 'LOCAL' ( LQx ; .. ; LQy ) 'SEP' () '|' ( SQx ; .. ; SQy )" :=
+  (mk_funspec (pair nil tz) cc_default ⊤ (atomic_spec_type W T)
+   (rev_curry (tcurry (λne x1, .. (tcurry (λne xn, tcurry (λne (Q : T -> mpred) (_ : tuple_type tnil),
      PROPx nil
      (PARAMSx nil (GLOBALSx (cons Gx .. (cons Gy nil) ..)
-     (SEPx (cons (atomic_shift (fun x => S2) (⊤ ∖ E) ∅ (fun x r => fold_right_sepcon (cons SQx%logic .. (cons SQy%logic nil) ..)) Q) nil))))))) ..)))
-   (fun (ts: list Type) => rev_curry (tcurry (fun x1 => .. (tcurry (fun xn => tcurry (fun (Q : T -> mpred) (_ : tuple_type tnil) =>
-    @exp (environ -> mpred) _ T (fun r =>
+     (SEPx (cons (atomic_shift (fun x => S2) (⊤ ∖ E) ∅ (fun x r => fold_right_sepcon (cons SQx%I .. (cons SQy%I nil) ..)) Q) nil))))))) ..)))
+   (rev_curry (tcurry (λne x1, .. (tcurry (λne xn, tcurry (λne (Q : T -> mpred) (_ : tuple_type tnil),
+    bi_exist(A := T) (fun r =>
      PROP () (LOCALx (cons LQx .. (cons LQy nil) ..) ((SEPx (Q r :: nil)))))))) ..)))
-   (@atomic_spec_nonexpansive_pre' _ T _ W
-      (fun (ts: list Type) => rev_curry (tcurry (fun x1 => .. (tcurry (fun xn (_ : tuple_type tnil) => nil)) ..)))
-      (fun (ts: list Type) => rev_curry (tcurry (fun x1 => .. (tcurry (fun xn (_ : tuple_type tnil) => nil)) ..)))
-      (fun (ts: list Type) => rev_curry (tcurry (fun x1 => .. (tcurry (fun xn (_ : tuple_type tnil) => (cons Gx .. (cons Gy nil) ..))) ..)))
-      (fun (ts: list Type) => rev_curry (tcurry (fun x1 => .. (tcurry (fun xn (_ : tuple_type tnil) => nil)) ..)))
-      (fun (ts: list Type) => rev_curry (tcurry (fun x1 => .. (tcurry (fun xn (_ : tuple_type tnil) x => S2)) ..)))       (fun (ts: list Type) => rev_curry (tcurry (fun x1 => .. (tcurry (fun xn (_ : tuple_type tnil) => E)) ..)))
-      (fun (ts: list Type) => rev_curry (tcurry (fun x1 => .. (tcurry (fun xn (_ : tuple_type tnil) x r => fold_right_sepcon (cons SQx%logic .. (cons SQy%logic nil) ..))) ..)))
-     _ _ _ _ _ _ _)
-  (atomic_spec_nonexpansive_post' W
-      (fun (ts: list Type) => rev_curry (tcurry (fun x1 => .. (tcurry (fun xn (_ : tuple_type tnil) r => (cons LQx%assert3 .. (cons LQy%assert3 nil) ..))) ..)))
-      (fun (ts: list Type) => rev_curry (tcurry (fun x1 => .. (tcurry (fun xn (_ : tuple_type tnil) r => nil)) ..))) _ _))
+   )
   (at level 200, x1 closed binder, xn closed binder, x at level 0, E at level 0, S2 at level 0, r at level 0, T at level 0).
 
-Notation "'ATOMIC' 'TYPE' W 'OBJ' x 'INVS' E 'WITH' x1 , .. , xn 'PRE'  [ ] 'PROP' ( Px ; .. ; Py ) 'PARAMS' () 'GLOBALS' ( Gx ; .. ; Gy ) 'SEP' ( S1x ; .. ; S1y ) '|' S2 'POST' [ tz ] 'EX' r : T , 'PROP' () 'LOCAL' () 'SEP' ( SPx ; .. ; SPy ) '|' ( SQx ; .. ; SQy )" :=
-  (mk_funspec (pair nil tz) cc_default (atomic_spec_type W T)
-   (fun (ts: list Type) => rev_curry (tcurry (fun x1 => .. (tcurry (fun xn => tcurry (fun (Q : T -> mpred) (_ : tuple_type tnil) =>
+Notation "'ATOMIC' 'TYPE' W 'OBJ' x 'INVS' E 'WITH' x1 , .. , xn 'PRE'  [ ] 'PROP' ( Px ; .. ; Py ) 'PARAMS' () 'GLOBALS' ( Gx ; .. ; Gy ) 'SEP' ( S1x ; .. ; S1y ) '|' S2 'POST' [ tz ] '∃' r : T , 'PROP' () 'LOCAL' () 'SEP' ( SPx ; .. ; SPy ) '|' ( SQx ; .. ; SQy )" :=
+  (mk_funspec (pair nil tz) cc_default ⊤ (atomic_spec_type W T)
+   (rev_curry (tcurry (λne x1, .. (tcurry (λne xn, tcurry (λne (Q : T -> mpred) (_ : tuple_type tnil),
      PROPx (cons Px%type .. (cons Py%type nil) ..)
      (PARAMSx nil (GLOBALSx (cons Gx .. (cons Gy nil) ..)
-     (SEPx (cons (atomic_shift (fun x => S2) (⊤ ∖ E) ∅ (fun x r => fold_right_sepcon (cons SQx%logic .. (cons SQy%logic nil) ..)) Q) (cons S1x%logic .. (cons S1y%logic nil) ..)))))))) ..)))
-   (fun (ts: list Type) => rev_curry (tcurry (fun x1 => .. (tcurry (fun xn => tcurry (fun (Q : T -> mpred) (_ : tuple_type tnil) =>
-    @exp (environ -> mpred) _ T (fun r =>
+     (SEPx (cons (atomic_shift (fun x => S2) (⊤ ∖ E) ∅ (fun x r => fold_right_sepcon (cons SQx%I .. (cons SQy%I nil) ..)) Q) (cons S1x%I .. (cons S1y%I nil) ..)))))))) ..)))
+   (rev_curry (tcurry (λne x1, .. (tcurry (λne xn, tcurry (λne (Q : T -> mpred) (_ : tuple_type tnil),
+    bi_exist(A := T) (fun r =>
      PROP () (LOCAL () (SEPx (Q r :: cons SPx .. (cons SPy nil) ..))))))) ..)))
-   (@atomic_spec_nonexpansive_pre' _ T _ W
-      (fun (ts: list Type) => rev_curry (tcurry (fun x1 => .. (tcurry (fun xn (_ : tuple_type tnil) => (cons Px%type .. (cons Py%type nil) ..))) ..)))
-      (fun (ts: list Type) => rev_curry (tcurry (fun x1 => .. (tcurry (fun xn (_ : tuple_type tnil) => nil)) ..)))
-      (fun (ts: list Type) => rev_curry (tcurry (fun x1 => .. (tcurry (fun xn (_ : tuple_type tnil) => (cons Gx .. (cons Gy nil) ..))) ..)))
-      (fun (ts: list Type) => rev_curry (tcurry (fun x1 => .. (tcurry (fun xn (_ : tuple_type tnil) => (cons S1x%logic .. (cons S1y%logic nil) ..))) ..)))
-      (fun (ts: list Type) => rev_curry (tcurry (fun x1 => .. (tcurry (fun xn (_ : tuple_type tnil) x => S2)) ..)))       (fun (ts: list Type) => rev_curry (tcurry (fun x1 => .. (tcurry (fun xn (_ : tuple_type tnil) => E)) ..)))
-      (fun (ts: list Type) => rev_curry (tcurry (fun x1 => .. (tcurry (fun xn (_ : tuple_type tnil) x r => fold_right_sepcon (cons SQx%logic .. (cons SQy%logic nil) ..))) ..)))
-     _ _ _ _ _ _ _)
-  (atomic_spec_nonexpansive_post' W
-      (fun (ts: list Type) => rev_curry (tcurry (fun x1 => .. (tcurry (fun xn (_ : tuple_type tnil) r => nil)) ..)))
-      (fun (ts: list Type) => rev_curry (tcurry (fun x1 => .. (tcurry (fun xn (_ : tuple_type tnil) r => (cons SPx%assert5%assert3 .. (cons SPy%assert5%assert3 nil) ..))) ..))) _ _))
-  (at level 200, x1 closed binder, xn closed binder, x at level 0, E at level 0, S2 at level 0, r at level 0, T at level 0).
-
-Notation "'ATOMIC' 'TYPE' W 'OBJ' x 'INVS' E 'WITH' x1 , .. , xn 'PRE'  [ ] 'PROP' ( Px ; .. ; Py ) 'PARAMS' () 'GLOBALS' ( Gx ; .. ; Gy ) 'SEP' ( S1x ; .. ; S1y ) '|' S2 'POST' [ tz ] 'PROP' () 'LOCAL' ( LQx ; .. ; LQy ) 'SEP' ( SPx ; .. ; SPy ) '|' ( SQx ; .. ; SQy )" :=
-  (mk_funspec (pair nil tz) cc_default (atomic_spec_type0 W)
-   (fun (ts: list Type) => rev_curry (tcurry (fun x1 => .. (tcurry (fun xn => tcurry (fun (Q : mpred) (_ : tuple_type tnil) =>
-     PROPx (cons Px%type .. (cons Py%type nil) ..)
-     (PARAMSx nil (GLOBALSx (cons Gx .. (cons Gy nil) ..)
-     (SEPx (cons (atomic_shift(B := unit) (fun x => S2) (⊤ ∖ E) ∅ (fun x _ => fold_right_sepcon (cons SQx%logic .. (cons SQy%logic nil) ..)) (fun _ => Q)) (cons S1x%logic .. (cons S1y%logic nil) ..)))))))) ..)))
-   (fun (ts: list Type) => rev_curry (tcurry (fun x1 => .. (tcurry (fun xn => tcurry (fun (Q : mpred) (_ : tuple_type tnil) =>
-     PROP () (LOCALx (cons LQx .. (cons LQy nil) ..) (SEPx (Q :: cons SPx .. (cons SPy nil) ..)))))) ..)))
-   (@atomic_spec_nonexpansive_pre0 _ W
-      (fun (ts: list Type) => rev_curry (tcurry (fun x1 => .. (tcurry (fun xn (_ : tuple_type tnil) => (cons Px%type .. (cons Py%type nil) ..))) ..)))
-      (fun (ts: list Type) => rev_curry (tcurry (fun x1 => .. (tcurry (fun xn (_ : tuple_type tnil) => nil)) ..)))
-      (fun (ts: list Type) => rev_curry (tcurry (fun x1 => .. (tcurry (fun xn (_ : tuple_type tnil) => (cons Gx .. (cons Gy nil) ..))) ..)))
-      (fun (ts: list Type) => rev_curry (tcurry (fun x1 => .. (tcurry (fun xn (_ : tuple_type tnil) => (cons S1x%logic .. (cons S1y%logic nil) ..))) ..)))
-      (fun (ts: list Type) => rev_curry (tcurry (fun x1 => .. (tcurry (fun xn (_ : tuple_type tnil) x => S2)) ..)))       (fun (ts: list Type) => rev_curry (tcurry (fun x1 => .. (tcurry (fun xn (_ : tuple_type tnil) => E)) ..)))
-      (fun (ts: list Type) => rev_curry (tcurry (fun x1 => .. (tcurry (fun xn (_ : tuple_type tnil) x _ => fold_right_sepcon (cons SQx%logic .. (cons SQy%logic nil) ..))) ..)))
-     _ _ _ _ _ _ _)
-  (atomic_spec_nonexpansive_post0 W
-      (fun (ts: list Type) => rev_curry (tcurry (fun x1 => .. (tcurry (fun xn (_ : tuple_type tnil) => (cons LQx%assert3 .. (cons LQy%assert3 nil) ..))) ..)))
-      (fun (ts: list Type) => rev_curry (tcurry (fun x1 => .. (tcurry (fun xn (_ : tuple_type tnil) => (cons SPx%assert3 .. (cons SPy%assert3 nil) ..))) ..))) _ _))
+   )
   (at level 200, x1 closed binder, xn closed binder, x at level 0, E at level 0, S2 at level 0).
 
 Notation "'ATOMIC' 'TYPE' W 'OBJ' x 'INVS' E 'WITH' x1 , .. , xn 'PRE'  [ ] 'PROP' ( Px ; .. ; Py ) 'PARAMS' () 'GLOBALS' ( Gx ; .. ; Gy ) 'SEP' ( S1x ; .. ; S1y ) '|' S2 'POST' [ tz ] 'PROP' () 'LOCAL' () 'SEP' ( SPx ; .. ; SPy ) '|' ( SQx ; .. ; SQy )" :=
-  (mk_funspec (pair nil tz) cc_default (atomic_spec_type0 W)
-   (fun (ts: list Type) => rev_curry (tcurry (fun x1 => .. (tcurry (fun xn => tcurry (fun (Q : mpred) (_ : tuple_type tnil) =>
-     PROPx (cons Px%type .. (cons Py%type nil) ..)
+  (mk_funspec (pair nil tz) cc_default ⊤ (atomic_spec_type0 W)
+   (rev_curry (tcurry (λne x1, .. (tcurry (λne xn, tcurry (λne (Q : mpred) (_ : tuple_type tnil),  PROPx (cons Px%type .. (cons Py%type nil) ..)
      (PARAMSx nil (GLOBALSx (cons Gx .. (cons Gy nil) ..)
-     (SEPx (cons (atomic_shift(B := unit) (fun x => S2) (⊤ ∖ E) ∅ (fun x _ => fold_right_sepcon (cons SQx%logic .. (cons SQy%logic nil) ..)) (fun _ => Q)) (cons S1x%logic .. (cons S1y%logic nil) ..)))))))) ..)))
-   (fun (ts: list Type) => rev_curry (tcurry (fun x1 => .. (tcurry (fun xn => tcurry (fun (Q : mpred) (_ : tuple_type tnil) =>
-     PROP () LOCAL () (SEPx (Q :: cons SPx .. (cons SPy nil) ..))))) ..)))
-   (@atomic_spec_nonexpansive_pre0 _ W
-      (fun (ts: list Type) => rev_curry (tcurry (fun x1 => .. (tcurry (fun xn (_ : tuple_type tnil) => (cons Px%type .. (cons Py%type nil) ..))) ..)))
-      (fun (ts: list Type) => rev_curry (tcurry (fun x1 => .. (tcurry (fun xn (_ : tuple_type tnil) => nil)) ..)))
-      (fun (ts: list Type) => rev_curry (tcurry (fun x1 => .. (tcurry (fun xn (_ : tuple_type tnil) => (cons Gx .. (cons Gy nil) ..))) ..)))
-      (fun (ts: list Type) => rev_curry (tcurry (fun x1 => .. (tcurry (fun xn (_ : tuple_type tnil) => (cons S1x%logic .. (cons S1y%logic nil) ..))) ..)))
-      (fun (ts: list Type) => rev_curry (tcurry (fun x1 => .. (tcurry (fun xn (_ : tuple_type tnil) x => S2)) ..)))       (fun (ts: list Type) => rev_curry (tcurry (fun x1 => .. (tcurry (fun xn (_ : tuple_type tnil) => E)) ..)))
-      (fun (ts: list Type) => rev_curry (tcurry (fun x1 => .. (tcurry (fun xn (_ : tuple_type tnil) x _ => fold_right_sepcon (cons SQx%logic .. (cons SQy%logic nil) ..))) ..)))
-     _ _ _ _ _ _ _)
-  (atomic_spec_nonexpansive_post0 W
-      (fun (ts: list Type) => rev_curry (tcurry (fun x1 => .. (tcurry (fun xn (_ : tuple_type tnil) => nil)) ..)))
-      (fun (ts: list Type) => rev_curry (tcurry (fun x1 => .. (tcurry (fun xn (_ : tuple_type tnil) => (cons SPx%assert5%assert3 .. (cons SPy%assert5%assert3 nil) ..))) ..))) _ _))
+     (SEPx (cons (atomic_shift(B := unit) (fun x => S2) (⊤ ∖ E) ∅ (fun x _ => fold_right_sepcon (cons SQx%I .. (cons SQy%I nil) ..)) (fun _ => Q)) (cons S1x%I .. (cons S1y%I nil) ..)))))))) ..)))
+   (rev_curry (tcurry (λne x1, .. (tcurry (λne xn, tcurry (λne (Q : mpred) (_ : tuple_type tnil),  PROP () LOCAL () (SEPx (Q :: cons SPx .. (cons SPy nil) ..))))) ..)))
+   )
   (at level 200, x1 closed binder, xn closed binder, x at level 0, E at level 0, S2 at level 0).
 
 Notation "'ATOMIC' 'TYPE' W 'OBJ' x 'INVS' E 'WITH' x1 , .. , xn 'PRE'  [ ] 'PROP' () 'PARAMS' () 'GLOBALS' ( Gx ; .. ; Gy ) 'SEP' () '|' S2 'POST' [ tz ] 'PROP' () 'LOCAL' ( LQx ; .. ; LQy ) 'SEP' () '|' ( SQx ; .. ; SQy )" :=
-  (mk_funspec (pair nil tz) cc_default (atomic_spec_type0 W)
-   (fun (ts: list Type) => rev_curry (tcurry (fun x1 => .. (tcurry (fun xn => tcurry (fun (Q : mpred) (_ : tuple_type tnil) =>
-     PROPx nil
+  (mk_funspec (pair nil tz) cc_default ⊤ (atomic_spec_type0 W)
+   (rev_curry (tcurry (λne x1, .. (tcurry (λne xn, tcurry (λne (Q : mpred) (_ : tuple_type tnil),  PROPx nil
      (PARAMSx nil (GLOBALSx (cons Gx .. (cons Gy nil) ..)
-     (SEPx (cons (atomic_shift(B := unit) (fun x => S2) (⊤ ∖ E) ∅ (fun x _ => fold_right_sepcon (cons SQx%logic .. (cons SQy%logic nil) ..)) (fun _ => Q)) nil))))))) ..)))
-   (fun (ts: list Type) => rev_curry (tcurry (fun x1 => .. (tcurry (fun xn => tcurry (fun (Q : mpred) (_ : tuple_type tnil) =>
-     PROP () (LOCALx (cons LQx .. (cons LQy nil) ..) (SEPx (Q :: nil)))))) ..)))
-   (@atomic_spec_nonexpansive_pre0 _ W
-      (fun (ts: list Type) => rev_curry (tcurry (fun x1 => .. (tcurry (fun xn (_ : tuple_type tnil) => nil)) ..)))
-      (fun (ts: list Type) => rev_curry (tcurry (fun x1 => .. (tcurry (fun xn (_ : tuple_type tnil) => nil)) ..)))
-      (fun (ts: list Type) => rev_curry (tcurry (fun x1 => .. (tcurry (fun xn (_ : tuple_type tnil) => (cons Gx .. (cons Gy nil) ..))) ..)))
-      (fun (ts: list Type) => rev_curry (tcurry (fun x1 => .. (tcurry (fun xn (_ : tuple_type tnil) => nil)) ..)))
-      (fun (ts: list Type) => rev_curry (tcurry (fun x1 => .. (tcurry (fun xn (_ : tuple_type tnil) x => S2)) ..)))       (fun (ts: list Type) => rev_curry (tcurry (fun x1 => .. (tcurry (fun xn (_ : tuple_type tnil) => E)) ..)))
-      (fun (ts: list Type) => rev_curry (tcurry (fun x1 => .. (tcurry (fun xn (_ : tuple_type tnil) x _ => fold_right_sepcon (cons SQx%logic .. (cons SQy%logic nil) ..))) ..)))
-     _ _ _ _ _ _ _)
-  (atomic_spec_nonexpansive_post0 W
-      (fun (ts: list Type) => rev_curry (tcurry (fun x1 => .. (tcurry (fun xn (_ : tuple_type tnil) => (cons LQx%assert3 .. (cons LQy%assert3 nil) ..))) ..)))
-      (fun (ts: list Type) => rev_curry (tcurry (fun x1 => .. (tcurry (fun xn (_ : tuple_type tnil) => nil)) ..))) _ _))
+     (SEPx (cons (atomic_shift(B := unit) (fun x => S2) (⊤ ∖ E) ∅ (fun x _ => fold_right_sepcon (cons SQx%I .. (cons SQy%I nil) ..)) (fun _ => Q)) nil))))))) ..)))
+   (rev_curry (tcurry (λne x1, .. (tcurry (λne xn, tcurry (λne (Q : mpred) (_ : tuple_type tnil),  PROP () (LOCALx (cons LQx .. (cons LQy nil) ..) (SEPx (Q :: nil)))))) ..)))
+   )
   (at level 200, x1 closed binder, xn closed binder, x at level 0, E at level 0, S2 at level 0).
 
 Notation "'ATOMIC' 'TYPE' W 'OBJ' x 'INVS' E 'WITH' x1 , .. , xn 'PRE'  [ ] 'PROP' () 'PARAMS' () 'GLOBALS' ( Gx ; .. ; Gy ) 'SEP' () '|' S2 'POST' [ tz ] 'PROP' () 'LOCAL' () 'SEP' () '|' ( SQx ; .. ; SQy )" :=
-  (mk_funspec (pair nil tz) cc_default (atomic_spec_type0 W)
-   (fun (ts: list Type) => rev_curry (tcurry (fun x1 => .. (tcurry (fun xn => tcurry (fun (Q : mpred) (_ : tuple_type tnil) =>
-     PROPx nil
+  (mk_funspec (pair nil tz) cc_default ⊤ (atomic_spec_type0 W)
+   (rev_curry (tcurry (λne x1, .. (tcurry (λne xn, tcurry (λne (Q : mpred) (_ : tuple_type tnil),  PROPx nil
      (PARAMSx nil (GLOBALSx (cons Gx .. (cons Gy nil) ..)
-     (SEPx (cons (atomic_shift(B := unit) (fun x => S2) (⊤ ∖ E) ∅ (fun x _ => fold_right_sepcon (cons SQx%logic .. (cons SQy%logic nil) ..)) (fun _ => Q)) nil))))))) ..)))
-   (fun (ts: list Type) => rev_curry (tcurry (fun x1 => .. (tcurry (fun xn => tcurry (fun (Q : mpred) (_ : tuple_type tnil) =>
-     PROP () LOCAL () (SEPx (Q :: nil))))) ..)))
-   (@atomic_spec_nonexpansive_pre0 _ W
-      (fun (ts: list Type) => rev_curry (tcurry (fun x1 => .. (tcurry (fun xn (_ : tuple_type tnil) => nil)) ..)))
-      (fun (ts: list Type) => rev_curry (tcurry (fun x1 => .. (tcurry (fun xn (_ : tuple_type tnil) => nil)) ..)))
-      (fun (ts: list Type) => rev_curry (tcurry (fun x1 => .. (tcurry (fun xn (_ : tuple_type tnil) => (cons Gx .. (cons Gy nil) ..))) ..)))
-      (fun (ts: list Type) => rev_curry (tcurry (fun x1 => .. (tcurry (fun xn (_ : tuple_type tnil) => nil)) ..)))
-      (fun (ts: list Type) => rev_curry (tcurry (fun x1 => .. (tcurry (fun xn (_ : tuple_type tnil) x => S2)) ..)))       (fun (ts: list Type) => rev_curry (tcurry (fun x1 => .. (tcurry (fun xn (_ : tuple_type tnil) => E)) ..)))
-      (fun (ts: list Type) => rev_curry (tcurry (fun x1 => .. (tcurry (fun xn (_ : tuple_type tnil) x _ => fold_right_sepcon (cons SQx%logic .. (cons SQy%logic nil) ..))) ..)))
-     _ _ _ _ _ _ _)
-  (atomic_spec_nonexpansive_post0 W
-      (fun (ts: list Type) => rev_curry (tcurry (fun x1 => .. (tcurry (fun xn (_ : tuple_type tnil) => nil)) ..)))
-      (fun (ts: list Type) => rev_curry (tcurry (fun x1 => .. (tcurry (fun xn (_ : tuple_type tnil) => nil)) ..))) _ _))
+     (SEPx (cons (atomic_shift(B := unit) (fun x => S2) (⊤ ∖ E) ∅ (fun x _ => fold_right_sepcon (cons SQx%I .. (cons SQy%I nil) ..)) (fun _ => Q)) nil))))))) ..)))
+   (rev_curry (tcurry (λne x1, .. (tcurry (λne xn, tcurry (λne (Q : mpred) (_ : tuple_type tnil),  PROP () LOCAL () (SEPx (Q :: nil))))) ..)))
+   )
   (at level 200, x1 closed binder, xn closed binder, x at level 0, E at level 0, S2 at level 0).
 
 Notation "'ATOMIC' 'TYPE' W 'INVS' E 'WITH' x1 , .. , xn 'PRE'  [ u , .. , v ] 'PROP' () 'PARAMS' ( Lx ; .. ; Ly ) 'GLOBALS' ( Gx ; .. ; Gy ) 'SEP' ( S1x ; .. ; S1y ) '|' S2 'POST' [ tz ] 'PROP' () 'LOCAL' () 'SEP' ( SPx ; .. ; SPy ) '|' ( SQx ; .. ; SQy )" :=
-  (mk_funspec (pair (cons u%type .. (cons v%type nil) ..) tz) cc_default (atomic_spec_type0 W)
-   (fun (ts: list Type) => rev_curry (tcurry (fun x1 => .. (tcurry (fun xn => tcurry (fun (Q : mpred) (_ : tuple_type tnil) =>
-     PROPx nil
+  (mk_funspec (pair (cons u%type .. (cons v%type nil) ..) tz) cc_default ⊤ (atomic_spec_type0 W)
+   (rev_curry (tcurry (λne x1, .. (tcurry (λne xn, tcurry (λne (Q : mpred) (_ : tuple_type tnil),  PROPx nil
      (PARAMSx (cons Lx%type .. (cons Ly%type nil) ..) (GLOBALSx (cons Gx .. (cons Gy nil) ..)
-     (SEPx (cons (atomic_shift(B := unit) (fun _ : unit => S2) (⊤ ∖ E) ∅ (fun _ _ => fold_right_sepcon (cons SQx%logic .. (cons SQy%logic nil) ..)) (fun _ => Q)) (cons S1x%logic .. (cons S1y%logic nil) ..)))))))) ..)))
-   (fun (ts: list Type) => rev_curry (tcurry (fun x1 => .. (tcurry (fun xn => tcurry (fun (Q : mpred) (_ : tuple_type tnil) =>
-     PROP () LOCAL () (SEPx (Q :: cons SPx .. (cons SPy nil) ..))))) ..)))
-   (@atomic_spec_nonexpansive_pre0 _ W
-      (fun (ts: list Type) => rev_curry (tcurry (fun x1 => .. (tcurry (fun xn (_ : tuple_type tnil) => nil)) ..)))
-      (fun (ts: list Type) => rev_curry (tcurry (fun x1 => .. (tcurry (fun xn (_ : tuple_type tnil) => (cons Lx%type .. (cons Ly%type nil) ..))) ..)))
-      (fun (ts: list Type) => rev_curry (tcurry (fun x1 => .. (tcurry (fun xn (_ : tuple_type tnil) => (cons Gx .. (cons Gy nil) ..))) ..)))
-      (fun (ts: list Type) => rev_curry (tcurry (fun x1 => .. (tcurry (fun xn (_ : tuple_type tnil) => (cons S1x%logic .. (cons S1y%logic nil) ..))) ..)))
-      (fun (ts: list Type) => rev_curry (tcurry (fun x1 => .. (tcurry (fun xn (_ : tuple_type tnil) (_:unit) => S2)) ..)))       (fun (ts: list Type) => rev_curry (tcurry (fun x1 => .. (tcurry (fun xn (_ : tuple_type tnil) => E)) ..)))
-      (fun (ts: list Type) => rev_curry (tcurry (fun x1 => .. (tcurry (fun xn (_ : tuple_type tnil) _ _ => fold_right_sepcon (cons SQx%logic .. (cons SQy%logic nil) ..))) ..)))
-     _ _ _ _ _ _ _)
-  (atomic_spec_nonexpansive_post0 W
-      (fun (ts: list Type) => rev_curry (tcurry (fun x1 => .. (tcurry (fun xn (_ : tuple_type tnil) => nil)) ..)))
-      (fun (ts: list Type) => rev_curry (tcurry (fun x1 => .. (tcurry (fun xn (_ : tuple_type tnil) => (cons SPx%assert5%assert3 .. (cons SPy%assert5%assert3 nil) ..))) ..))) _ _))
+     (SEPx (cons (atomic_shift(B := unit) (fun _ : unit => S2) (⊤ ∖ E) ∅ (fun _ _ => fold_right_sepcon (cons SQx%I .. (cons SQy%I nil) ..)) (fun _ => Q)) (cons S1x%I .. (cons S1y%I nil) ..)))))))) ..)))
+   (rev_curry (tcurry (λne x1, .. (tcurry (λne xn, tcurry (λne (Q : mpred) (_ : tuple_type tnil),  PROP () LOCAL () (SEPx (Q :: cons SPx .. (cons SPy nil) ..))))) ..)))
+   )
   (at level 200, x1 closed binder, xn closed binder, E at level 0, S2 at level 0).
 
 Notation "'ATOMIC' 'TYPE' W 'OBJ' x 'INVS' E 'WITH' x1 , .. , xn 'PRE'  [ u , .. , v ] 'PROP' () 'PARAMS' ( Lx ; .. ; Ly ) 'GLOBALS' ( Gx ; .. ; Gy ) 'SEP' ( S1x ; .. ; S1y ) '|' S2 'POST' [ tz ] 'PROP' () 'LOCAL' () 'SEP' ( SPx ; .. ; SPy ) '|' ( SQx ; .. ; SQy )" :=
-  (mk_funspec (pair (cons u%type .. (cons v%type nil) ..) tz) cc_default (atomic_spec_type0 W)
-   (fun (ts: list Type) => rev_curry (tcurry (fun x1 => .. (tcurry (fun xn => tcurry (fun (Q : mpred) (_ : tuple_type tnil) =>
-     PROPx nil
+  (mk_funspec (pair (cons u%type .. (cons v%type nil) ..) tz) cc_default ⊤ (atomic_spec_type0 W)
+   (rev_curry (tcurry (λne x1, .. (tcurry (λne xn, tcurry (λne (Q : mpred) (_ : tuple_type tnil),  PROPx nil
      (PARAMSx (cons Lx%type .. (cons Ly%type nil) ..) (GLOBALSx (cons Gx .. (cons Gy nil) ..)
-     (SEPx (cons (atomic_shift(B := unit) (fun x => S2) (⊤ ∖ E) ∅ (fun x _ => fold_right_sepcon (cons SQx%logic .. (cons SQy%logic nil) ..)) (fun _ => Q)) (cons S1x%logic .. (cons S1y%logic nil) ..)))))))) ..)))
-   (fun (ts: list Type) => rev_curry (tcurry (fun x1 => .. (tcurry (fun xn => tcurry (fun (Q : mpred) (_ : tuple_type tnil) =>
-     PROP () LOCAL () (SEPx (Q :: cons SPx .. (cons SPy nil) ..))))) ..)))
-   (@atomic_spec_nonexpansive_pre0 _ W
-      (fun (ts: list Type) => rev_curry (tcurry (fun x1 => .. (tcurry (fun xn (_ : tuple_type tnil) => nil)) ..)))
-      (fun (ts: list Type) => rev_curry (tcurry (fun x1 => .. (tcurry (fun xn (_ : tuple_type tnil) => (cons Lx%type .. (cons Ly%type nil) ..))) ..)))
-      (fun (ts: list Type) => rev_curry (tcurry (fun x1 => .. (tcurry (fun xn (_ : tuple_type tnil) => (cons Gx .. (cons Gy nil) ..))) ..)))
-      (fun (ts: list Type) => rev_curry (tcurry (fun x1 => .. (tcurry (fun xn (_ : tuple_type tnil) => (cons S1x%logic .. (cons S1y%logic nil) ..))) ..)))
-      (fun (ts: list Type) => rev_curry (tcurry (fun x1 => .. (tcurry (fun xn (_ : tuple_type tnil) x => S2)) ..)))       (fun (ts: list Type) => rev_curry (tcurry (fun x1 => .. (tcurry (fun xn (_ : tuple_type tnil) => E)) ..)))
-      (fun (ts: list Type) => rev_curry (tcurry (fun x1 => .. (tcurry (fun xn (_ : tuple_type tnil) x _ => fold_right_sepcon (cons SQx%logic .. (cons SQy%logic nil) ..))) ..)))
-     _ _ _ _ _ _ _)
-  (atomic_spec_nonexpansive_post0 W
-      (fun (ts: list Type) => rev_curry (tcurry (fun x1 => .. (tcurry (fun xn (_ : tuple_type tnil) => nil)) ..)))
-      (fun (ts: list Type) => rev_curry (tcurry (fun x1 => .. (tcurry (fun xn (_ : tuple_type tnil) => (cons SPx%assert5%assert3 .. (cons SPy%assert5%assert3 nil) ..))) ..))) _ _))
+     (SEPx (cons (atomic_shift(B := unit) (fun x => S2) (⊤ ∖ E) ∅ (fun x _ => fold_right_sepcon (cons SQx%I .. (cons SQy%I nil) ..)) (fun _ => Q)) (cons S1x%I .. (cons S1y%I nil) ..)))))))) ..)))
+   (rev_curry (tcurry (λne x1, .. (tcurry (λne xn, tcurry (λne (Q : mpred) (_ : tuple_type tnil),  PROP () LOCAL () (SEPx (Q :: cons SPx .. (cons SPy nil) ..))))) ..)))
+   )
   (at level 200, x1 closed binder, xn closed binder, x at level 0, E at level 0, S2 at level 0).
 
 Notation "'ATOMIC' 'TYPE' W 'INVS' E 'WITH' x1 , .. , xn 'PRE'  [ u , .. , v ] 'PROP' () 'PARAMS' ( Lx ; .. ; Ly ) 'SEP' () '|' S2 'POST' [ tz ] 'PROP' () 'LOCAL' () 'SEP' () '|' ( SQx ; .. ; SQy )" :=
-  (mk_funspec (pair (cons u%type .. (cons v%type nil) ..) tz) cc_default (atomic_spec_type0 W)
-   (fun (ts: list Type) => rev_curry (tcurry (fun x1 => .. (tcurry (fun xn => tcurry (fun (Q : mpred) (_ : tuple_type tnil) =>
-     PROPx nil
+  (mk_funspec (pair (cons u%type .. (cons v%type nil) ..) tz) cc_default ⊤ (atomic_spec_type0 W)
+   (rev_curry (tcurry (λne x1, .. (tcurry (λne xn, tcurry (λne (Q : mpred) (_ : tuple_type tnil),  PROPx nil
      (PARAMSx (cons Lx%type .. (cons Ly%type nil) ..) (GLOBALSx nil
-     (SEPx (cons (atomic_shift(B := unit) (fun _ : unit => S2) (⊤ ∖ E) ∅ (fun _ _ => fold_right_sepcon (cons SQx%logic .. (cons SQy%logic nil) ..)) (fun _ => Q)) nil))))))) ..)))
-   (fun (ts: list Type) => rev_curry (tcurry (fun x1 => .. (tcurry (fun xn => tcurry (fun (Q : mpred) (_ : tuple_type tnil) =>
-     PROP () LOCAL () (SEPx (Q :: nil))))) ..)))
-   (@atomic_spec_nonexpansive_pre0 _ W
-      (fun (ts: list Type) => rev_curry (tcurry (fun x1 => .. (tcurry (fun xn (_ : tuple_type tnil) => nil)) ..)))
-      (fun (ts: list Type) => rev_curry (tcurry (fun x1 => .. (tcurry (fun xn (_ : tuple_type tnil) => (cons Lx%type .. (cons Ly%type nil) ..))) ..)))
-      (fun (ts: list Type) => rev_curry (tcurry (fun x1 => .. (tcurry (fun xn (_ : tuple_type tnil) => nil)) ..)))
-      (fun (ts: list Type) => rev_curry (tcurry (fun x1 => .. (tcurry (fun xn (_ : tuple_type tnil) => nil)) ..)))
-      (fun (ts: list Type) => rev_curry (tcurry (fun x1 => .. (tcurry (fun xn (_ : tuple_type tnil) (_:unit) => S2)) ..)))       (fun (ts: list Type) => rev_curry (tcurry (fun x1 => .. (tcurry (fun xn (_ : tuple_type tnil) => E)) ..)))
-      (fun (ts: list Type) => rev_curry (tcurry (fun x1 => .. (tcurry (fun xn (_ : tuple_type tnil) _ _ => fold_right_sepcon (cons SQx%logic .. (cons SQy%logic nil) ..))) ..)))
-     _ _ _ _ _ _ _)
-  (atomic_spec_nonexpansive_post0 W
-      (fun (ts: list Type) => rev_curry (tcurry (fun x1 => .. (tcurry (fun xn (_ : tuple_type tnil) => nil)) ..)))
-      (fun (ts: list Type) => rev_curry (tcurry (fun x1 => .. (tcurry (fun xn (_ : tuple_type tnil) => nil)) ..))) _ _))
+     (SEPx (cons (atomic_shift(B := unit) (fun _ : unit => S2) (⊤ ∖ E) ∅ (fun _ _ => fold_right_sepcon (cons SQx%I .. (cons SQy%I nil) ..)) (fun _ => Q)) nil))))))) ..)))
+   (rev_curry (tcurry (λne x1, .. (tcurry (λne xn, tcurry (λne (Q : mpred) (_ : tuple_type tnil),  PROP () LOCAL () (SEPx (Q :: nil))))) ..)))
+   )
   (at level 200, x1 closed binder, xn closed binder, E at level 0, S2 at level 0).
 
 Notation "'ATOMIC' 'TYPE' W 'OBJ' x 'INVS' E 'WITH' x1 , .. , xn 'PRE'  [ u , .. , v ] 'PROP' () 'PARAMS' ( Lx ; .. ; Ly ) 'SEP' () '|' S2 'POST' [ tz ] 'PROP' () 'LOCAL' () 'SEP' () '|' ( SQx ; .. ; SQy )" :=
-  (mk_funspec (pair (cons u%type .. (cons v%type nil) ..) tz) cc_default (atomic_spec_type0 W)
-   (fun (ts: list Type) => rev_curry (tcurry (fun x1 => .. (tcurry (fun xn => tcurry (fun (Q : mpred) (_ : tuple_type tnil) =>
-     PROPx nil
+  (mk_funspec (pair (cons u%type .. (cons v%type nil) ..) tz) cc_default ⊤ (atomic_spec_type0 W)
+   (rev_curry (tcurry (λne x1, .. (tcurry (λne xn, tcurry (λne (Q : mpred) (_ : tuple_type tnil),  PROPx nil
      (PARAMSx (cons Lx%type .. (cons Ly%type nil) ..) (GLOBALSx nil
-     (SEPx (cons (atomic_shift(B := unit) (fun x => S2) (⊤ ∖ E) ∅ (fun x _ => fold_right_sepcon (cons SQx%logic .. (cons SQy%logic nil) ..)) (fun _ => Q)) nil))))))) ..)))
-   (fun (ts: list Type) => rev_curry (tcurry (fun x1 => .. (tcurry (fun xn => tcurry (fun (Q : mpred) (_ : tuple_type tnil) =>
-     PROP () LOCAL () (SEPx (Q :: nil))))) ..)))
-   (@atomic_spec_nonexpansive_pre0 _ W
-      (fun (ts: list Type) => rev_curry (tcurry (fun x1 => .. (tcurry (fun xn (_ : tuple_type tnil) => nil)) ..)))
-      (fun (ts: list Type) => rev_curry (tcurry (fun x1 => .. (tcurry (fun xn (_ : tuple_type tnil) => (cons Lx%type .. (cons Ly%type nil) ..))) ..)))
-      (fun (ts: list Type) => rev_curry (tcurry (fun x1 => .. (tcurry (fun xn (_ : tuple_type tnil) => nil)) ..)))
-      (fun (ts: list Type) => rev_curry (tcurry (fun x1 => .. (tcurry (fun xn (_ : tuple_type tnil) => nil)) ..)))
-      (fun (ts: list Type) => rev_curry (tcurry (fun x1 => .. (tcurry (fun xn (_ : tuple_type tnil) x => S2)) ..)))
-      (fun (ts: list Type) => rev_curry (tcurry (fun x1 => .. (tcurry (fun xn (_ : tuple_type tnil) => E)) ..)))
-      (fun (ts: list Type) => rev_curry (tcurry (fun x1 => .. (tcurry (fun xn (_ : tuple_type tnil) x _ => fold_right_sepcon (cons SQx%logic .. (cons SQy%logic nil) ..))) ..)))
-     _ _ _ _ _ _ _)
-  (atomic_spec_nonexpansive_post0 W
-      (fun (ts: list Type) => rev_curry (tcurry (fun x1 => .. (tcurry (fun xn (_ : tuple_type tnil) => nil)) ..)))
-      (fun (ts: list Type) => rev_curry (tcurry (fun x1 => .. (tcurry (fun xn (_ : tuple_type tnil) => nil)) ..))) _ _))
+     (SEPx (cons (atomic_shift(B := unit) (fun x => S2) (⊤ ∖ E) ∅ (fun x _ => fold_right_sepcon (cons SQx%I .. (cons SQy%I nil) ..)) (fun _ => Q)) nil))))))) ..)))
+   (rev_curry (tcurry (λne x1, .. (tcurry (λne xn, tcurry (λne (Q : mpred) (_ : tuple_type tnil),  PROP () LOCAL () (SEPx (Q :: nil))))) ..)))
+   )
   (at level 200, x1 closed binder, xn closed binder, x at level 0, E at level 0, S2 at level 0).
 
 Notation "'ATOMIC' 'TYPE' W 'OBJ' x 'INVS' E 'WITH' x1 , .. , xn 'PRE'  [ u , .. , v ] 'PROP' () 'PARAMS' ( Lx ; .. ; Ly ) 'SEP' ( S1x ; .. ; S1y ) '|' S2 'POST' [ tz ] 'PROP' () 'LOCAL' () 'SEP' () '|' ( SQx ; .. ; SQy )" :=
-  (mk_funspec (pair (cons u%type .. (cons v%type nil) ..) tz) cc_default (atomic_spec_type0 W)
-   (fun (ts: list Type) => rev_curry (tcurry (fun x1 => .. (tcurry (fun xn => tcurry (fun (Q : mpred) (_ : tuple_type tnil) =>
-     PROPx nil
+  (mk_funspec (pair (cons u%type .. (cons v%type nil) ..) tz) cc_default ⊤ (atomic_spec_type0 W)
+   (rev_curry (tcurry (λne x1, .. (tcurry (λne xn, tcurry (λne (Q : mpred) (_ : tuple_type tnil),  PROPx nil
      (PARAMSx (cons Lx%type .. (cons Ly%type nil) ..) (GLOBALSx nil
-     (SEPx (cons (atomic_shift(B := unit) (fun x => S2) (⊤ ∖ E) ∅ (fun x _ => fold_right_sepcon (cons SQx%logic .. (cons SQy%logic nil) ..)) (fun _ => Q)) (cons S1x%logic .. (cons S1y%logic nil) ..)))))))) ..)))
-   (fun (ts: list Type) => rev_curry (tcurry (fun x1 => .. (tcurry (fun xn => tcurry (fun (Q : mpred) (_ : tuple_type tnil) =>
-     PROP () LOCAL () (SEPx (Q :: nil))))) ..)))
-   (@atomic_spec_nonexpansive_pre0 _ W
-      (fun (ts: list Type) => rev_curry (tcurry (fun x1 => .. (tcurry (fun xn (_ : tuple_type tnil) => nil)) ..)))
-      (fun (ts: list Type) => rev_curry (tcurry (fun x1 => .. (tcurry (fun xn (_ : tuple_type tnil) => (cons Lx%type .. (cons Ly%type nil) ..))) ..)))
-      (fun (ts: list Type) => rev_curry (tcurry (fun x1 => .. (tcurry (fun xn (_ : tuple_type tnil) => nil)) ..)))
-      (fun (ts: list Type) => rev_curry (tcurry (fun x1 => .. (tcurry (fun xn (_ : tuple_type tnil) => (cons S1x%logic .. (cons S1y%logic nil) ..))) ..)))
-      (fun (ts: list Type) => rev_curry (tcurry (fun x1 => .. (tcurry (fun xn (_ : tuple_type tnil) x => S2)) ..)))
-      (fun (ts: list Type) => rev_curry (tcurry (fun x1 => .. (tcurry (fun xn (_ : tuple_type tnil) => E)) ..)))
-      (fun (ts: list Type) => rev_curry (tcurry (fun x1 => .. (tcurry (fun xn (_ : tuple_type tnil) x _ => fold_right_sepcon (cons SQx%logic .. (cons SQy%logic nil) ..))) ..)))
-     _ _ _ _ _ _ _)
-  (atomic_spec_nonexpansive_post0 W
-      (fun (ts: list Type) => rev_curry (tcurry (fun x1 => .. (tcurry (fun xn (_ : tuple_type tnil) => nil)) ..)))
-      (fun (ts: list Type) => rev_curry (tcurry (fun x1 => .. (tcurry (fun xn (_ : tuple_type tnil) => nil)) ..))) _ _))
+     (SEPx (cons (atomic_shift(B := unit) (fun x => S2) (⊤ ∖ E) ∅ (fun x _ => fold_right_sepcon (cons SQx%I .. (cons SQy%I nil) ..)) (fun _ => Q)) (cons S1x%I .. (cons S1y%I nil) ..)))))))) ..)))
+   (rev_curry (tcurry (λne x1, .. (tcurry (λne xn, tcurry (λne (Q : mpred) (_ : tuple_type tnil),  PROP () LOCAL () (SEPx (Q :: nil))))) ..)))
+   )
   (at level 200, x1 closed binder, xn closed binder, x at level 0, E at level 0, S2 at level 0).
 
 Notation "'ATOMIC' 'TYPE' W 'OBJ' x 'INVS' E 'WITH' x1 , .. , xn 'PRE'  [ u , .. , v ] 'PROP' () 'PARAMS' ( Lx ; .. ; Ly ) 'SEP' ( S1x ; .. ; S1y ) '|' S2 'POST' [ tz ] 'PROP' () 'LOCAL' () 'SEP' ( SPx ; .. ; SPy ) '|' ( SQx ; .. ; SQy )" :=
-  (mk_funspec (pair (cons u%type .. (cons v%type nil) ..) tz) cc_default (atomic_spec_type0 W)
-   (fun (ts: list Type) => rev_curry (tcurry (fun x1 => .. (tcurry (fun xn => tcurry (fun (Q : mpred) (_ : tuple_type tnil) =>
-     PROPx nil
+  (mk_funspec (pair (cons u%type .. (cons v%type nil) ..) tz) cc_default ⊤ (atomic_spec_type0 W)
+   (rev_curry (tcurry (λne x1, .. (tcurry (λne xn, tcurry (λne (Q : mpred) (_ : tuple_type tnil),  PROPx nil
      (PARAMSx (cons Lx%type .. (cons Ly%type nil) ..) (GLOBALSx nil
-     (SEPx (cons (atomic_shift(B := unit) (fun x => S2) (⊤ ∖ E) ∅ (fun x _ => fold_right_sepcon (cons SQx%logic .. (cons SQy%logic nil) ..)) (fun _ => Q)) (cons S1x%logic .. (cons S1y%logic nil) ..)))))))) ..)))
-   (fun (ts: list Type) => rev_curry (tcurry (fun x1 => .. (tcurry (fun xn => tcurry (fun (Q : mpred) (_ : tuple_type tnil) =>
-     PROP () LOCAL () (SEPx (Q :: cons SPx .. (cons SPy nil) ..))))) ..)))
-   (@atomic_spec_nonexpansive_pre0 _ W
-      (fun (ts: list Type) => rev_curry (tcurry (fun x1 => .. (tcurry (fun xn (_ : tuple_type tnil) => nil)) ..)))
-      (fun (ts: list Type) => rev_curry (tcurry (fun x1 => .. (tcurry (fun xn (_ : tuple_type tnil) => (cons Lx%type .. (cons Ly%type nil) ..))) ..)))
-      (fun (ts: list Type) => rev_curry (tcurry (fun x1 => .. (tcurry (fun xn (_ : tuple_type tnil) => nil)) ..)))
-      (fun (ts: list Type) => rev_curry (tcurry (fun x1 => .. (tcurry (fun xn (_ : tuple_type tnil) => (cons S1x%logic .. (cons S1y%logic nil) ..))) ..)))
-      (fun (ts: list Type) => rev_curry (tcurry (fun x1 => .. (tcurry (fun xn (_ : tuple_type tnil) x => S2)) ..)))
-      (fun (ts: list Type) => rev_curry (tcurry (fun x1 => .. (tcurry (fun xn (_ : tuple_type tnil) => E)) ..)))
-      (fun (ts: list Type) => rev_curry (tcurry (fun x1 => .. (tcurry (fun xn (_ : tuple_type tnil) x _ => fold_right_sepcon (cons SQx%logic .. (cons SQy%logic nil) ..))) ..)))
-     _ _ _ _ _ _ _)
-  (atomic_spec_nonexpansive_post0 W
-      (fun (ts: list Type) => rev_curry (tcurry (fun x1 => .. (tcurry (fun xn (_ : tuple_type tnil) => nil)) ..)))
-      (fun (ts: list Type) => rev_curry (tcurry (fun x1 => .. (tcurry (fun xn (_ : tuple_type tnil) => cons SPx%assert5%assert3 .. (cons SPy%assert5%assert3 nil) ..)) ..))) _ _))
+     (SEPx (cons (atomic_shift(B := unit) (fun x => S2) (⊤ ∖ E) ∅ (fun x _ => fold_right_sepcon (cons SQx%I .. (cons SQy%I nil) ..)) (fun _ => Q)) (cons S1x%I .. (cons S1y%I nil) ..)))))))) ..)))
+   (rev_curry (tcurry (λne x1, .. (tcurry (λne xn, tcurry (λne (Q : mpred) (_ : tuple_type tnil),  PROP () LOCAL () (SEPx (Q :: cons SPx .. (cons SPy nil) ..))))) ..)))
+   )
   (at level 200, x1 closed binder, xn closed binder, x at level 0, E at level 0, S2 at level 0).
 
 Notation "'ATOMIC' 'TYPE' W 'INVS' E 'WITH' x1 , .. , xn 'PRE'  [ u , .. , v ] 'PROP' () 'PARAMS' ( Lx ; .. ; Ly ) 'SEP' ( S1x ; .. ; S1y ) '|' S2 'POST' [ tz ] 'PROP' () 'LOCAL' () 'SEP' ( SPx ; .. ; SPy ) '|' ( SQx ; .. ; SQy )" :=
-  (mk_funspec (pair (cons u%type .. (cons v%type nil) ..) tz) cc_default (atomic_spec_type0 W)
-   (fun (ts: list Type) => rev_curry (tcurry (fun x1 => .. (tcurry (fun xn => tcurry (fun (Q : mpred) (_ : tuple_type tnil) =>
-     PROPx nil
+  (mk_funspec (pair (cons u%type .. (cons v%type nil) ..) tz) cc_default ⊤ (atomic_spec_type0 W)
+   (rev_curry (tcurry (λne x1, .. (tcurry (λne xn, tcurry (λne (Q : mpred) (_ : tuple_type tnil),  PROPx nil
      (PARAMSx (cons Lx%type .. (cons Ly%type nil) ..) (GLOBALSx nil
-     (SEPx (cons (atomic_shift(B := unit) (fun (_ : unit) => S2) (⊤ ∖ E) ∅ (fun (_ : unit) _ => fold_right_sepcon (cons SQx%logic .. (cons SQy%logic nil) ..)) (fun _ => Q)) (cons S1x%logic .. (cons S1y%logic nil) ..)))))))) ..)))
-   (fun (ts: list Type) => rev_curry (tcurry (fun x1 => .. (tcurry (fun xn => tcurry (fun (Q : mpred) (_ : tuple_type tnil) =>
-     PROP () LOCAL () (SEPx (Q :: cons SPx .. (cons SPy nil) ..))))) ..)))
-   (@atomic_spec_nonexpansive_pre0 _ W
-      (fun (ts: list Type) => rev_curry (tcurry (fun x1 => .. (tcurry (fun xn (_ : tuple_type tnil) => nil)) ..)))
-      (fun (ts: list Type) => rev_curry (tcurry (fun x1 => .. (tcurry (fun xn (_ : tuple_type tnil) => (cons Lx%type .. (cons Ly%type nil) ..))) ..)))
-      (fun (ts: list Type) => rev_curry (tcurry (fun x1 => .. (tcurry (fun xn (_ : tuple_type tnil) => nil)) ..)))
-      (fun (ts: list Type) => rev_curry (tcurry (fun x1 => .. (tcurry (fun xn (_ : tuple_type tnil) => (cons S1x%logic .. (cons S1y%logic nil) ..))) ..)))
-      (fun (ts: list Type) => rev_curry (tcurry (fun x1 => .. (tcurry (fun xn (_ : tuple_type tnil) (_ : unit) => S2)) ..)))
-      (fun (ts: list Type) => rev_curry (tcurry (fun x1 => .. (tcurry (fun xn (_ : tuple_type tnil) => E)) ..)))
-      (fun (ts: list Type) => rev_curry (tcurry (fun x1 => .. (tcurry (fun xn (_ : tuple_type tnil) (_ : unit) _ => fold_right_sepcon (cons SQx%logic .. (cons SQy%logic nil) ..))) ..)))
-     _ _ _ _ _ _ _)
-  (atomic_spec_nonexpansive_post0 W
-      (fun (ts: list Type) => rev_curry (tcurry (fun x1 => .. (tcurry (fun xn (_ : tuple_type tnil) => nil)) ..)))
-      (fun (ts: list Type) => rev_curry (tcurry (fun x1 => .. (tcurry (fun xn (_ : tuple_type tnil) => cons SPx%assert5%assert3 .. (cons SPy%assert5%assert3 nil) ..)) ..))) _ _))
+     (SEPx (cons (atomic_shift(B := unit) (fun (_ : unit) => S2) (⊤ ∖ E) ∅ (fun (_ : unit) _ => fold_right_sepcon (cons SQx%I .. (cons SQy%I nil) ..)) (fun _ => Q)) (cons S1x%I .. (cons S1y%I nil) ..)))))))) ..)))
+   (rev_curry (tcurry (λne x1, .. (tcurry (λne xn, tcurry (λne (Q : mpred) (_ : tuple_type tnil),  PROP () LOCAL () (SEPx (Q :: cons SPx .. (cons SPy nil) ..))))) ..)))
+   )
   (at level 200, x1 closed binder, xn closed binder, E at level 0, S2 at level 0).
 
 Notation "'ATOMIC' 'TYPE' W 'INVS' E 'WITH' x1 , .. , xn 'PRE'  [ u , .. , v ] 'PROP' ( Px ; .. ; Py ) 'PARAMS' ( Lx ; .. ; Ly ) 'SEP' ( S1x ; .. ; S1y ) '|' S2 'POST' [ tz ] 'PROP' () 'LOCAL' () 'SEP' ( SPx ; .. ; SPy ) '|' ( SQx ; .. ; SQy )" :=
-  (mk_funspec (pair (cons u%type .. (cons v%type nil) ..) tz) cc_default (atomic_spec_type0 W)
-   (fun (ts: list Type) => rev_curry (tcurry (fun x1 => .. (tcurry (fun xn => tcurry (fun (Q : mpred) (_ : tuple_type tnil) =>
-     PROPx (cons Px%type .. (cons Py%type nil) ..)
+  (mk_funspec (pair (cons u%type .. (cons v%type nil) ..) tz) cc_default ⊤ (atomic_spec_type0 W)
+   (rev_curry (tcurry (λne x1, .. (tcurry (λne xn, tcurry (λne (Q : mpred) (_ : tuple_type tnil),  PROPx (cons Px%type .. (cons Py%type nil) ..)
      (PARAMSx (cons Lx%type .. (cons Ly%type nil) ..) (GLOBALSx nil
-     (SEPx (cons (atomic_shift(B := unit) (fun (_ : unit) => S2) (⊤ ∖ E) ∅ (fun (_ : unit) _ => fold_right_sepcon (cons SQx%logic .. (cons SQy%logic nil) ..)) (fun _ => Q)) (cons S1x%logic .. (cons S1y%logic nil) ..)))))))) ..)))
-   (fun (ts: list Type) => rev_curry (tcurry (fun x1 => .. (tcurry (fun xn => tcurry (fun (Q : mpred) (_ : tuple_type tnil) =>
-     PROP () LOCAL () (SEPx (Q :: cons SPx .. (cons SPy nil) ..))))) ..)))
-   (@atomic_spec_nonexpansive_pre0 _ W
-      (fun (ts: list Type) => rev_curry (tcurry (fun x1 => .. (tcurry (fun xn (_ : tuple_type tnil) => cons Px%type .. (cons Py%type nil) ..)) ..)))
-      (fun (ts: list Type) => rev_curry (tcurry (fun x1 => .. (tcurry (fun xn (_ : tuple_type tnil) => (cons Lx%type .. (cons Ly%type nil) ..))) ..)))
-      (fun (ts: list Type) => rev_curry (tcurry (fun x1 => .. (tcurry (fun xn (_ : tuple_type tnil) => nil)) ..)))
-      (fun (ts: list Type) => rev_curry (tcurry (fun x1 => .. (tcurry (fun xn (_ : tuple_type tnil) => (cons S1x%logic .. (cons S1y%logic nil) ..))) ..)))
-      (fun (ts: list Type) => rev_curry (tcurry (fun x1 => .. (tcurry (fun xn (_ : tuple_type tnil) (_ : unit) => S2)) ..)))
-      (fun (ts: list Type) => rev_curry (tcurry (fun x1 => .. (tcurry (fun xn (_ : tuple_type tnil) => E)) ..)))
-      (fun (ts: list Type) => rev_curry (tcurry (fun x1 => .. (tcurry (fun xn (_ : tuple_type tnil) (_ : unit) _ => fold_right_sepcon (cons SQx%logic .. (cons SQy%logic nil) ..))) ..)))
-     _ _ _ _ _ _ _)
-  (atomic_spec_nonexpansive_post0 W
-      (fun (ts: list Type) => rev_curry (tcurry (fun x1 => .. (tcurry (fun xn (_ : tuple_type tnil) => nil)) ..)))
-      (fun (ts: list Type) => rev_curry (tcurry (fun x1 => .. (tcurry (fun xn (_ : tuple_type tnil) => cons SPx%assert5%assert3 .. (cons SPy%assert5%assert3 nil) ..)) ..))) _ _))
+     (SEPx (cons (atomic_shift(B := unit) (fun (_ : unit) => S2) (⊤ ∖ E) ∅ (fun (_ : unit) _ => fold_right_sepcon (cons SQx%I .. (cons SQy%I nil) ..)) (fun _ => Q)) (cons S1x%I .. (cons S1y%I nil) ..)))))))) ..)))
+   (rev_curry (tcurry (λne x1, .. (tcurry (λne xn, tcurry (λne (Q : mpred) (_ : tuple_type tnil),  PROP () LOCAL () (SEPx (Q :: cons SPx .. (cons SPy nil) ..))))) ..)))
+   )
   (at level 200, x1 closed binder, xn closed binder, E at level 0, S2 at level 0).
 
 Notation "'ATOMIC' 'TYPE' W 'OBJ' x 'INVS' E 'WITH' x1 , .. , xn 'PRE'  [ u , .. , v ] 'PROP' ( Px ; .. ; Py ) 'PARAMS' ( Lx ; .. ; Ly ) 'SEP' ( S1x ; .. ; S1y ) '|' S2 'POST' [ tz ] 'PROP' () 'LOCAL' () 'SEP' ( SPx ; .. ; SPy ) '|' ( SQx ; .. ; SQy )" :=
-  (mk_funspec (pair (cons u%type .. (cons v%type nil) ..) tz) cc_default (atomic_spec_type0 W)
-   (fun (ts: list Type) => rev_curry (tcurry (fun x1 => .. (tcurry (fun xn => tcurry (fun (Q : mpred) (_ : tuple_type tnil) =>
-     PROPx (cons Px%type .. (cons Py%type nil) ..)
+  (mk_funspec (pair (cons u%type .. (cons v%type nil) ..) tz) cc_default ⊤ (atomic_spec_type0 W)
+   (rev_curry (tcurry (λne x1, .. (tcurry (λne xn, tcurry (λne (Q : mpred) (_ : tuple_type tnil),  PROPx (cons Px%type .. (cons Py%type nil) ..)
      (PARAMSx (cons Lx%type .. (cons Ly%type nil) ..) (GLOBALSx nil
-     (SEPx (cons (atomic_shift(B := unit) (fun x => S2) (⊤ ∖ E) ∅ (fun x _ => fold_right_sepcon (cons SQx%logic .. (cons SQy%logic nil) ..)) (fun _ => Q)) (cons S1x%logic .. (cons S1y%logic nil) ..)))))))) ..)))
-   (fun (ts: list Type) => rev_curry (tcurry (fun x1 => .. (tcurry (fun xn => tcurry (fun (Q : mpred) (_ : tuple_type tnil) =>
-     PROP () LOCAL () (SEPx (Q :: cons SPx .. (cons SPy nil) ..))))) ..)))
-   (@atomic_spec_nonexpansive_pre0 _ W
-      (fun (ts: list Type) => rev_curry (tcurry (fun x1 => .. (tcurry (fun xn (_ : tuple_type tnil) => (cons Px%type .. (cons Py%type nil) ..))) ..)))
-      (fun (ts: list Type) => rev_curry (tcurry (fun x1 => .. (tcurry (fun xn (_ : tuple_type tnil) => (cons Lx%type .. (cons Ly%type nil) ..))) ..)))
-      (fun (ts: list Type) => rev_curry (tcurry (fun x1 => .. (tcurry (fun xn (_ : tuple_type tnil) => nil)) ..)))
-      (fun (ts: list Type) => rev_curry (tcurry (fun x1 => .. (tcurry (fun xn (_ : tuple_type tnil) => (cons S1x%logic .. (cons S1y%logic nil) ..))) ..)))
-      (fun (ts: list Type) => rev_curry (tcurry (fun x1 => .. (tcurry (fun xn (_ : tuple_type tnil) x => S2)) ..)))
-      (fun (ts: list Type) => rev_curry (tcurry (fun x1 => .. (tcurry (fun xn (_ : tuple_type tnil) => E)) ..)))
-      (fun (ts: list Type) => rev_curry (tcurry (fun x1 => .. (tcurry (fun xn (_ : tuple_type tnil) x _ => fold_right_sepcon (cons SQx%logic .. (cons SQy%logic nil) ..))) ..)))
-     _ _ _ _ _ _ _)
-  (atomic_spec_nonexpansive_post0 W
-      (fun (ts: list Type) => rev_curry (tcurry (fun x1 => .. (tcurry (fun xn (_ : tuple_type tnil) => nil)) ..)))
-      (fun (ts: list Type) => rev_curry (tcurry (fun x1 => .. (tcurry (fun xn (_ : tuple_type tnil) => cons SPx%assert5%assert3 .. (cons SPy%assert5%assert3 nil) ..)) ..))) _ _))
+     (SEPx (cons (atomic_shift(B := unit) (fun x => S2) (⊤ ∖ E) ∅ (fun x _ => fold_right_sepcon (cons SQx%I .. (cons SQy%I nil) ..)) (fun _ => Q)) (cons S1x%I .. (cons S1y%I nil) ..)))))))) ..)))
+   (rev_curry (tcurry (λne x1, .. (tcurry (λne xn, tcurry (λne (Q : mpred) (_ : tuple_type tnil),  PROP () LOCAL () (SEPx (Q :: cons SPx .. (cons SPy nil) ..))))) ..)))
+   )
   (at level 200, x1 closed binder, xn closed binder, x at level 0, E at level 0, S2 at level 0).
 
 
-Ltac atomic_nonexpansive_tac := try (let x := fresh "x" in intros ?? x;
+(*Ltac atomic_nonexpansive_tac := try (let x := fresh "x" in intros ?? x;
   try match type of x with list Type => (let ts := fresh "ts" in rename x into ts; intros x) end;
   repeat destruct x as [x ?]; unfold rev_curry, tcurry; simpl; auto); repeat constructor.
 
-Global Obligation Tactic := atomic_nonexpansive_tac.
+Global Obligation Tactic := atomic_nonexpansive_tac.*)
 
 (* change start_function to handle curried arguments -- also thanks to Jason *)
 Ltac read_names term :=
   lazymatch term with
-  | tcurry (fun x : ?T => ?f)
+  | tcurry (λne x : ?T, ?f)
     => let f' := fresh in
        let rest := lazymatch
              constr:(
-               fun x : T
-               => match f return _ with
+               λne x : T,
+                  match f return _ with
                   | f' => ltac:(let f := (eval cbv delta [f'] in f') in
                                 clear f';
                                 let rest := read_names f in
                                 refine rest)
                   end) with
-           | fun _ => ?rest => rest
+           | λne _, ?rest => rest
            | ?e => fail 0 "Could not eliminate the functional dependencies of" e
            end in
-       constr:(((fun x : unit => x), rest))
+       constr:(((λne x : unit, x), rest))
   | _ => constr:(tt)
   end.
 
 Ltac destruct_args t i :=
   match t with
   | tt => idtac
-  | (fun x => _, ?t') => destruct_args t' i; (destruct i as [i x] || rename i into x)
+  | (λne x, _, ?t') => destruct_args t' i; (destruct i as [i x] || rename i into x)
   end.
 
 Ltac start_function1 ::=
  leaf_function;
- lazymatch goal with |- semax_body ?V ?G ?F ?spec =>
-    check_normalized F;
-    function_body_unsupported_features F;
-    let s := fresh "spec" in
-    pose (s:=spec); hnf in s; cbn zeta in s; (* dependent specs defined with Program Definition often have extra lets *)
-   repeat lazymatch goal with
-    | s := (_, NDmk_funspec _ _ _ _ _) |- _ => fail
-    | s := (_, mk_funspec _ _ _ _ _ _ _) |- _ => fail
-    | s := (_, ?a _ _ _ _) |- _ => unfold a in s
-    | s := (_, ?a _ _ _) |- _ => unfold a in s
-    | s := (_, ?a _ _) |- _ => unfold a in s
-    | s := (_, ?a _) |- _ => unfold a in s
-    | s := (_, ?a) |- _ => unfold a in s
+   lazymatch goal with
+   | |- semax_body ?V ?G ?F ?spec =>
+         check_normalized F; function_body_unsupported_features F;
+          (let s := fresh "spec" in
+           pose (s := spec); hnf in s; cbn zeta in s;
+            repeat
+             lazymatch goal with
+             | s:=(_, NDmk_funspec _ _ _ _ _):_ |- _ => fail
+             | s:=(_, mk_funspec _ _ _ _ _ _):_ |- _ => fail
+             | s:=(_, ?a _ _ _ _):_ |- _ => unfold a in s
+             | s:=(_, ?a _ _ _):_ |- _ => unfold a in s
+             | s:=(_, ?a _ _):_ |- _ => unfold a in s
+             | s:=(_, ?a _):_ |- _ => unfold a in s
+             | s:=(_, ?a):_ |- _ => unfold a in s
+             end;
+            lazymatch goal with
+            | s:=(_, WITH _ : globals PRE [ ] main_pre _ _ _ POST [tint] _):_
+              |- _ => idtac
+            | s:=?spec':_ |- _ => check_canonical_funspec spec'
+            end; change (semax_body V G F s); subst s)
+   end; unfold NDmk_funspec;
+   (let gv := fresh "gv" in
+    match goal with
+    | |- semax_body _ _ _ (_, mk_funspec _ _ _ _ ?Pre _) =>
+          split3; [ check_parameter_types' | check_return_type |  ];
+           match Pre with
+           | λne _, monPred_at (convertPre _ _ (λ i, _)) =>
+               intros Espec i
+           | λne x, monPred_at match _ with
+                               | (a, b) => _
+                               end => intros Espec [a b]
+           | λne i, _ => intros Espec i
+           end; simpl fn_body; simpl fn_params; simpl fn_return
     end;
-    lazymatch goal with
-    | s :=  (_,  WITH _: globals
-               PRE  [] main_pre _ _ _
-               POST [ tint ] _) |- _ => idtac
-    | s := ?spec' |- _ => check_canonical_funspec spec'
-   end;
-   change (semax_body V G F s); subst s;
-   unfold NDmk_funspec'
- end;
- let DependedTypeList := fresh "DependedTypeList" in
- unfold NDmk_funspec;
- match goal with |- semax_body _ _ _ (pair _ (mk_funspec _ _ _ ?Pre _ _ _)) =>
-
-   split3; [check_parameter_types' | check_return_type | ];
-    match Pre with
-   | (fun _ => rev_curry ?t) => let i := fresh in let x := read_names t in intros Espec DependedTypeList i; destruct_args x i; unfold rev_curry, tcurry; simpl tcurry_rev; cbn match (* added line *)
-   | (fun _ => convertPre _ _ (fun i => _)) =>  intros Espec DependedTypeList i
-   | (fun _ x => match _ with (a,b) => _ end) => intros Espec DependedTypeList [a b]
-   | (fun _ i => _) => intros Espec DependedTypeList i
-   end;
-   simpl fn_body; simpl fn_params; simpl fn_return
- end;
- try match goal with |- semax _ (fun rho => ?A rho * ?B rho)%logic _ _ =>
-     change (fun rho => ?A rho * ?B rho)%logic with (A * B)%logic
-  end;
- simpl functors.MixVariantFunctor._functor in *;
- simpl rmaps.dependent_type_functor_rec;
- clear DependedTypeList;
- rewrite_old_main_pre;
- repeat match goal with
- | |- @semax _ _ _ (match ?p with (a,b) => _ end * _)%logic _ _ =>
-             destruct p as [a b]
- | |- @semax _ _ _ (close_precondition _ match ?p with (a,b) => _ end * _) _ _ =>
-             destruct p as [a b]
- | |- @semax _ _ _ ((match ?p with (a,b) => _ end) eq_refl * _)%logic _ _ =>
-             destruct p as [a b]
- | |- @semax _ _ _ (close_precondition _ ((match ?p with (a,b) => _ end) eq_refl) * _) _ _ =>
-             destruct p as [a b]
- | |- semax _ (close_precondition _
-                                                (fun ae => !! (Datatypes.length (snd ae) = ?A) && ?B
-                                                      (make_args ?C (snd ae) (mkEnviron (fst ae) _ _))) * _)%logic _ _ =>
-          match B with match ?p with (a,b) => _ end => destruct p as [a b] end
-       end;
-(* this speeds things up, but only in the very rare case where it applies,
-   so maybe not worth it ...
-  repeat match goal with H: reptype _ |- _ => progress hnf in H; simpl in H; idtac "reduced a reptype" end;
-*)
- rewrite ?difference_empty_L; (* added line *)
- try start_func_convert_precondition.
+     cbv[dtfr dependent_type_functor_rec constOF idOF prodOF discrete_funOF ofe_morOF
+        sigTOF listOF oFunctor_car ofe_car] in *; cbv[ofe_mor_car];
+     rewrite_old_main_pre; rewrite ?argsassert_of_at ?assert_of_at;
+     repeat
+      match goal with
+      | |- semax _ _ (match ?p with
+                      | (a, b) => _
+                      end ∗ _) _ _ => destruct p as [a b]
+      | |- semax _ _ (close_precondition _ match ?p with
+                                           | (a, b) => _
+                                           end ∗ _) _ _ => 
+        destruct p as [a b]
+      | |-
+        semax _ _
+          (close_precondition _ (argsassert_of match ?p with
+                                               | (a, b) => _
+                                               end) ∗ _) _ _ => 
+        destruct p as [a b]
+      | |- semax _ _ (match ?p with
+                      | (a, b) => _
+                      end eq_refl ∗ _) _ _ => destruct p as [a b]
+      | |-
+        semax _ _
+          (close_precondition _ (match ?p with
+                                 | (a, b) => _
+                                 end eq_refl) ∗ _) _ _ => 
+        destruct p as [a b]
+      | |-
+        semax _ _
+          (close_precondition _
+             (argsassert_of (match ?p with
+                             | (a, b) => _
+                             end eq_refl)) ∗ _) _ _ => destruct p as [a b]
+      | |-
+        semax _ _
+          (close_precondition _
+             (λ ae,
+                ⌜Datatypes.length ae.2 = ?A⌝
+                ∧ ?B (make_args ?C ae.2 (mkEnviron ae.1 _ _))) ∗ _) _ _ =>
+            match B with
+            | match ?p with
+              | (a, b) => _
+              end => destruct p as [a b]
+            end
+      end; rewrite ?argsassert_of_at ?assert_of_at;
+     rewrite ?difference_empty_L; (* added line *)
+     try start_func_convert_precondition).
 
 (* can we not do this? *)
 Ltac start_function2 ::=
